Attempt to update ink submodule

CoqOfRust/ink/erc20.v
@@ -25,7 +25,7 @@ Module erc20.
   
   Definition ChainExtension : Set := ink_env.types.Environment.ChainExtension.
   
-  Definition MAX_EVENT_TOPICS `{H : State.Trait} : usize :=
+  Definition MAX_EVENT_TOPICS : usize :=
     run (Pure ink_env.types.Environment.MAX_EVENT_TOPICS).
   
   Module Erc20.
@@ -50,13 +50,10 @@ Module erc20.
   Module Impl_core_default_Default_for_erc20_erc20_Erc20.
     Definition Self := erc20.erc20.Erc20.
     
-    Definition default
-        `{H : State.Trait}
-        (_ : unit)
-        : M (H := H) erc20.erc20.Erc20 :=
-      let* α0 := core.default.Default.default tt in
-      let* α1 := core.default.Default.default tt in
-      let* α2 := core.default.Default.default tt in
+    Definition default  : M erc20.erc20.Erc20 :=
+      let* α0 := core.default.Default.default  in
+      let* α1 := core.default.Default.default  in
+      let* α2 := core.default.Default.default  in
       Pure
         {|
           erc20.erc20.Erc20.total_supply := α0;
@@ -64,13 +61,13 @@ Module erc20.
           erc20.erc20.Erc20.allowances := α2;
         |}.
     
-    Global Instance AssociatedFunction_default `{H : State.Trait} :
+    Global Instance AssociatedFunction_default :
       Notation.DoubleColon Self "default" := {
       Notation.double_colon := default;
     }.
     
     Global Instance I : core.default.Default.Trait Self := {
-      core.default.Default.default `{H : State.Trait} := default;
+      core.default.Default.default := default;
     }.
   End Impl_core_default_Default_for_erc20_erc20_Erc20.
   
@@ -152,7 +149,7 @@ Module erc20.
     Definition
       IS_RESULT := Pure ink.reflect.dispatch.ConstructorOutput.IS_RESULT.
     
-    Global Instance AssociatedFunction_IS_RESULT `{H : State.Trait} :
+    Global Instance AssociatedFunction_IS_RESULT :
       Notation.DoubleColon Self "IS_RESULT" := {
       Notation.double_colon := IS_RESULT;
     }.
@@ -161,54 +158,39 @@ Module erc20.
       CALLABLE := Pure
         (fun __ink_binding_0 => erc20.erc20.Erc20::["new"] __ink_binding_0).
     
-    Global Instance AssociatedFunction_CALLABLE `{H : State.Trait} :
+    Global Instance AssociatedFunction_CALLABLE :
       Notation.DoubleColon Self "CALLABLE" := {
       Notation.double_colon := CALLABLE;
     }.
     
     Definition PAYABLE := Pure false.
     
-    Global Instance AssociatedFunction_PAYABLE `{H : State.Trait} :
+    Global Instance AssociatedFunction_PAYABLE :
       Notation.DoubleColon Self "PAYABLE" := {
       Notation.double_colon := PAYABLE;
     }.
     
     Definition SELECTOR := Pure [ 155; 174; 157; 94 ].
     
-    Global Instance AssociatedFunction_SELECTOR `{H : State.Trait} :
+    Global Instance AssociatedFunction_SELECTOR :
       Notation.DoubleColon Self "SELECTOR" := {
       Notation.double_colon := SELECTOR;
     }.
     
     Definition LABEL := Pure "new".
     
-    Global Instance AssociatedFunction_LABEL `{H : State.Trait} :
+    Global Instance AssociatedFunction_LABEL :
       Notation.DoubleColon Self "LABEL" := {
       Notation.double_colon := LABEL;
     }.
     
     Global Instance I :
         ink.reflect.dispatch.DispatchableConstructorInfo.Trait Self := {
-      ink.reflect.dispatch.DispatchableConstructorInfo.IS_RESULT
-        `{H : State.Trait}
-        :=
-        IS_RESULT;
-      ink.reflect.dispatch.DispatchableConstructorInfo.CALLABLE
-        `{H : State.Trait}
-        :=
-        CALLABLE;
-      ink.reflect.dispatch.DispatchableConstructorInfo.PAYABLE
-        `{H : State.Trait}
-        :=
-        PAYABLE;
-      ink.reflect.dispatch.DispatchableConstructorInfo.SELECTOR
-        `{H : State.Trait}
-        :=
-        SELECTOR;
-      ink.reflect.dispatch.DispatchableConstructorInfo.LABEL
-        `{H : State.Trait}
-        :=
-        LABEL;
+      ink.reflect.dispatch.DispatchableConstructorInfo.IS_RESULT := IS_RESULT;
+      ink.reflect.dispatch.DispatchableConstructorInfo.CALLABLE := CALLABLE;
+      ink.reflect.dispatch.DispatchableConstructorInfo.PAYABLE := PAYABLE;
+      ink.reflect.dispatch.DispatchableConstructorInfo.SELECTOR := SELECTOR;
+      ink.reflect.dispatch.DispatchableConstructorInfo.LABEL := LABEL;
     }.
   End
     Impl_ink_reflect_dispatch_DispatchableConstructorInfo_for_erc20_erc20_Erc20.
@@ -227,61 +209,46 @@ Module erc20.
       CALLABLE := Pure
         (fun storage _ => erc20.erc20.Erc20::["total_supply"] storage).
     
-    Global Instance AssociatedFunction_CALLABLE `{H : State.Trait} :
+    Global Instance AssociatedFunction_CALLABLE :
       Notation.DoubleColon Self "CALLABLE" := {
       Notation.double_colon := CALLABLE;
     }.
     
     Definition SELECTOR := Pure [ 219; 99; 117; 168 ].
     
-    Global Instance AssociatedFunction_SELECTOR `{H : State.Trait} :
+    Global Instance AssociatedFunction_SELECTOR :
       Notation.DoubleColon Self "SELECTOR" := {
       Notation.double_colon := SELECTOR;
     }.
     
     Definition PAYABLE := Pure false.
     
-    Global Instance AssociatedFunction_PAYABLE `{H : State.Trait} :
+    Global Instance AssociatedFunction_PAYABLE :
       Notation.DoubleColon Self "PAYABLE" := {
       Notation.double_colon := PAYABLE;
     }.
     
     Definition MUTATES := Pure false.
     
-    Global Instance AssociatedFunction_MUTATES `{H : State.Trait} :
+    Global Instance AssociatedFunction_MUTATES :
       Notation.DoubleColon Self "MUTATES" := {
       Notation.double_colon := MUTATES;
     }.
     
     Definition LABEL := Pure "total_supply".
     
-    Global Instance AssociatedFunction_LABEL `{H : State.Trait} :
+    Global Instance AssociatedFunction_LABEL :
       Notation.DoubleColon Self "LABEL" := {
       Notation.double_colon := LABEL;
     }.
     
     Global Instance I :
         ink.reflect.dispatch.DispatchableMessageInfo.Trait Self := {
-      ink.reflect.dispatch.DispatchableMessageInfo.CALLABLE
-        `{H : State.Trait}
-        :=
-        CALLABLE;
-      ink.reflect.dispatch.DispatchableMessageInfo.MUTATES
-        `{H : State.Trait}
-        :=
-        MUTATES;
-      ink.reflect.dispatch.DispatchableMessageInfo.PAYABLE
-        `{H : State.Trait}
-        :=
-        PAYABLE;
-      ink.reflect.dispatch.DispatchableMessageInfo.SELECTOR
-        `{H : State.Trait}
-        :=
-        SELECTOR;
-      ink.reflect.dispatch.DispatchableMessageInfo.LABEL
-        `{H : State.Trait}
-        :=
-        LABEL;
+      ink.reflect.dispatch.DispatchableMessageInfo.CALLABLE := CALLABLE;
+      ink.reflect.dispatch.DispatchableMessageInfo.MUTATES := MUTATES;
+      ink.reflect.dispatch.DispatchableMessageInfo.PAYABLE := PAYABLE;
+      ink.reflect.dispatch.DispatchableMessageInfo.SELECTOR := SELECTOR;
+      ink.reflect.dispatch.DispatchableMessageInfo.LABEL := LABEL;
     }.
   End Impl_ink_reflect_dispatch_DispatchableMessageInfo_for_erc20_erc20_Erc20.
   
@@ -300,61 +267,46 @@ Module erc20.
         (fun storage __ink_binding_0 =>
           erc20.erc20.Erc20::["balance_of"] storage __ink_binding_0).
     
-    Global Instance AssociatedFunction_CALLABLE `{H : State.Trait} :
+    Global Instance AssociatedFunction_CALLABLE :
       Notation.DoubleColon Self "CALLABLE" := {
       Notation.double_colon := CALLABLE;
     }.
     
     Definition SELECTOR := Pure [ 15; 117; 90; 86 ].
     
-    Global Instance AssociatedFunction_SELECTOR `{H : State.Trait} :
+    Global Instance AssociatedFunction_SELECTOR :
       Notation.DoubleColon Self "SELECTOR" := {
       Notation.double_colon := SELECTOR;
     }.
     
     Definition PAYABLE := Pure false.
     
-    Global Instance AssociatedFunction_PAYABLE `{H : State.Trait} :
+    Global Instance AssociatedFunction_PAYABLE :
       Notation.DoubleColon Self "PAYABLE" := {
       Notation.double_colon := PAYABLE;
     }.
     
     Definition MUTATES := Pure false.
     
-    Global Instance AssociatedFunction_MUTATES `{H : State.Trait} :
+    Global Instance AssociatedFunction_MUTATES :
       Notation.DoubleColon Self "MUTATES" := {
       Notation.double_colon := MUTATES;
     }.
     
     Definition LABEL := Pure "balance_of".
     
-    Global Instance AssociatedFunction_LABEL `{H : State.Trait} :
+    Global Instance AssociatedFunction_LABEL :
       Notation.DoubleColon Self "LABEL" := {
       Notation.double_colon := LABEL;
     }.
     
     Global Instance I :
         ink.reflect.dispatch.DispatchableMessageInfo.Trait Self := {
-      ink.reflect.dispatch.DispatchableMessageInfo.CALLABLE
-        `{H : State.Trait}
-        :=
-        CALLABLE;
-      ink.reflect.dispatch.DispatchableMessageInfo.MUTATES
-        `{H : State.Trait}
-        :=
-        MUTATES;
-      ink.reflect.dispatch.DispatchableMessageInfo.PAYABLE
-        `{H : State.Trait}
-        :=
-        PAYABLE;
-      ink.reflect.dispatch.DispatchableMessageInfo.SELECTOR
-        `{H : State.Trait}
-        :=
-        SELECTOR;
-      ink.reflect.dispatch.DispatchableMessageInfo.LABEL
-        `{H : State.Trait}
-        :=
-        LABEL;
+      ink.reflect.dispatch.DispatchableMessageInfo.CALLABLE := CALLABLE;
+      ink.reflect.dispatch.DispatchableMessageInfo.MUTATES := MUTATES;
+      ink.reflect.dispatch.DispatchableMessageInfo.PAYABLE := PAYABLE;
+      ink.reflect.dispatch.DispatchableMessageInfo.SELECTOR := SELECTOR;
+      ink.reflect.dispatch.DispatchableMessageInfo.LABEL := LABEL;
     }.
   End Impl_ink_reflect_dispatch_DispatchableMessageInfo_for_erc20_erc20_Erc20.
   
@@ -376,61 +328,46 @@ Module erc20.
             __ink_binding_0
             __ink_binding_1).
     
-    Global Instance AssociatedFunction_CALLABLE `{H : State.Trait} :
+    Global Instance AssociatedFunction_CALLABLE :
       Notation.DoubleColon Self "CALLABLE" := {
       Notation.double_colon := CALLABLE;
     }.
     
     Definition SELECTOR := Pure [ 106; 0; 22; 94 ].
     
-    Global Instance AssociatedFunction_SELECTOR `{H : State.Trait} :
+    Global Instance AssociatedFunction_SELECTOR :
       Notation.DoubleColon Self "SELECTOR" := {
       Notation.double_colon := SELECTOR;
     }.
     
     Definition PAYABLE := Pure false.
     
-    Global Instance AssociatedFunction_PAYABLE `{H : State.Trait} :
+    Global Instance AssociatedFunction_PAYABLE :
       Notation.DoubleColon Self "PAYABLE" := {
       Notation.double_colon := PAYABLE;
     }.
     
     Definition MUTATES := Pure false.
     
-    Global Instance AssociatedFunction_MUTATES `{H : State.Trait} :
+    Global Instance AssociatedFunction_MUTATES :
       Notation.DoubleColon Self "MUTATES" := {
       Notation.double_colon := MUTATES;
     }.
     
     Definition LABEL := Pure "allowance".
     
-    Global Instance AssociatedFunction_LABEL `{H : State.Trait} :
+    Global Instance AssociatedFunction_LABEL :
       Notation.DoubleColon Self "LABEL" := {
       Notation.double_colon := LABEL;
     }.
     
     Global Instance I :
         ink.reflect.dispatch.DispatchableMessageInfo.Trait Self := {
-      ink.reflect.dispatch.DispatchableMessageInfo.CALLABLE
-        `{H : State.Trait}
-        :=
-        CALLABLE;
-      ink.reflect.dispatch.DispatchableMessageInfo.MUTATES
-        `{H : State.Trait}
-        :=
-        MUTATES;
-      ink.reflect.dispatch.DispatchableMessageInfo.PAYABLE
-        `{H : State.Trait}
-        :=
-        PAYABLE;
-      ink.reflect.dispatch.DispatchableMessageInfo.SELECTOR
-        `{H : State.Trait}
-        :=
-        SELECTOR;
-      ink.reflect.dispatch.DispatchableMessageInfo.LABEL
-        `{H : State.Trait}
-        :=
-        LABEL;
+      ink.reflect.dispatch.DispatchableMessageInfo.CALLABLE := CALLABLE;
+      ink.reflect.dispatch.DispatchableMessageInfo.MUTATES := MUTATES;
+      ink.reflect.dispatch.DispatchableMessageInfo.PAYABLE := PAYABLE;
+      ink.reflect.dispatch.DispatchableMessageInfo.SELECTOR := SELECTOR;
+      ink.reflect.dispatch.DispatchableMessageInfo.LABEL := LABEL;
     }.
   End Impl_ink_reflect_dispatch_DispatchableMessageInfo_for_erc20_erc20_Erc20.
   
@@ -452,61 +389,46 @@ Module erc20.
             __ink_binding_0
             __ink_binding_1).
     
-    Global Instance AssociatedFunction_CALLABLE `{H : State.Trait} :
+    Global Instance AssociatedFunction_CALLABLE :
       Notation.DoubleColon Self "CALLABLE" := {
       Notation.double_colon := CALLABLE;
     }.
     
     Definition SELECTOR := Pure [ 132; 161; 93; 161 ].
     
-    Global Instance AssociatedFunction_SELECTOR `{H : State.Trait} :
+    Global Instance AssociatedFunction_SELECTOR :
       Notation.DoubleColon Self "SELECTOR" := {
       Notation.double_colon := SELECTOR;
     }.
     
     Definition PAYABLE := Pure false.
     
-    Global Instance AssociatedFunction_PAYABLE `{H : State.Trait} :
+    Global Instance AssociatedFunction_PAYABLE :
       Notation.DoubleColon Self "PAYABLE" := {
       Notation.double_colon := PAYABLE;
     }.
     
     Definition MUTATES := Pure true.
     
-    Global Instance AssociatedFunction_MUTATES `{H : State.Trait} :
+    Global Instance AssociatedFunction_MUTATES :
       Notation.DoubleColon Self "MUTATES" := {
       Notation.double_colon := MUTATES;
     }.
     
     Definition LABEL := Pure "transfer".
     
-    Global Instance AssociatedFunction_LABEL `{H : State.Trait} :
+    Global Instance AssociatedFunction_LABEL :
       Notation.DoubleColon Self "LABEL" := {
       Notation.double_colon := LABEL;
     }.
     
     Global Instance I :
         ink.reflect.dispatch.DispatchableMessageInfo.Trait Self := {
-      ink.reflect.dispatch.DispatchableMessageInfo.CALLABLE
-        `{H : State.Trait}
-        :=
-        CALLABLE;
-      ink.reflect.dispatch.DispatchableMessageInfo.MUTATES
-        `{H : State.Trait}
-        :=
-        MUTATES;
-      ink.reflect.dispatch.DispatchableMessageInfo.PAYABLE
-        `{H : State.Trait}
-        :=
-        PAYABLE;
-      ink.reflect.dispatch.DispatchableMessageInfo.SELECTOR
-        `{H : State.Trait}
-        :=
-        SELECTOR;
-      ink.reflect.dispatch.DispatchableMessageInfo.LABEL
-        `{H : State.Trait}
-        :=
-        LABEL;
+      ink.reflect.dispatch.DispatchableMessageInfo.CALLABLE := CALLABLE;
+      ink.reflect.dispatch.DispatchableMessageInfo.MUTATES := MUTATES;
+      ink.reflect.dispatch.DispatchableMessageInfo.PAYABLE := PAYABLE;
+      ink.reflect.dispatch.DispatchableMessageInfo.SELECTOR := SELECTOR;
+      ink.reflect.dispatch.DispatchableMessageInfo.LABEL := LABEL;
     }.
   End Impl_ink_reflect_dispatch_DispatchableMessageInfo_for_erc20_erc20_Erc20.
   
@@ -528,61 +450,46 @@ Module erc20.
             __ink_binding_0
             __ink_binding_1).
     
-    Global Instance AssociatedFunction_CALLABLE `{H : State.Trait} :
+    Global Instance AssociatedFunction_CALLABLE :
       Notation.DoubleColon Self "CALLABLE" := {
       Notation.double_colon := CALLABLE;
     }.
     
     Definition SELECTOR := Pure [ 104; 18; 102; 160 ].
     
-    Global Instance AssociatedFunction_SELECTOR `{H : State.Trait} :
+    Global Instance AssociatedFunction_SELECTOR :
       Notation.DoubleColon Self "SELECTOR" := {
       Notation.double_colon := SELECTOR;
     }.
     
     Definition PAYABLE := Pure false.
     
-    Global Instance AssociatedFunction_PAYABLE `{H : State.Trait} :
+    Global Instance AssociatedFunction_PAYABLE :
       Notation.DoubleColon Self "PAYABLE" := {
       Notation.double_colon := PAYABLE;
     }.
     
     Definition MUTATES := Pure true.
     
-    Global Instance AssociatedFunction_MUTATES `{H : State.Trait} :
+    Global Instance AssociatedFunction_MUTATES :
       Notation.DoubleColon Self "MUTATES" := {
       Notation.double_colon := MUTATES;
     }.
     
     Definition LABEL := Pure "approve".
     
-    Global Instance AssociatedFunction_LABEL `{H : State.Trait} :
+    Global Instance AssociatedFunction_LABEL :
       Notation.DoubleColon Self "LABEL" := {
       Notation.double_colon := LABEL;
     }.
     
     Global Instance I :
         ink.reflect.dispatch.DispatchableMessageInfo.Trait Self := {
-      ink.reflect.dispatch.DispatchableMessageInfo.CALLABLE
-        `{H : State.Trait}
-        :=
-        CALLABLE;
-      ink.reflect.dispatch.DispatchableMessageInfo.MUTATES
-        `{H : State.Trait}
-        :=
-        MUTATES;
-      ink.reflect.dispatch.DispatchableMessageInfo.PAYABLE
-        `{H : State.Trait}
-        :=
-        PAYABLE;
-      ink.reflect.dispatch.DispatchableMessageInfo.SELECTOR
-        `{H : State.Trait}
-        :=
-        SELECTOR;
-      ink.reflect.dispatch.DispatchableMessageInfo.LABEL
-        `{H : State.Trait}
-        :=
-        LABEL;
+      ink.reflect.dispatch.DispatchableMessageInfo.CALLABLE := CALLABLE;
+      ink.reflect.dispatch.DispatchableMessageInfo.MUTATES := MUTATES;
+      ink.reflect.dispatch.DispatchableMessageInfo.PAYABLE := PAYABLE;
+      ink.reflect.dispatch.DispatchableMessageInfo.SELECTOR := SELECTOR;
+      ink.reflect.dispatch.DispatchableMessageInfo.LABEL := LABEL;
     }.
   End Impl_ink_reflect_dispatch_DispatchableMessageInfo_for_erc20_erc20_Erc20.
   
@@ -606,61 +513,46 @@ Module erc20.
             __ink_binding_1
             __ink_binding_2).
     
-    Global Instance AssociatedFunction_CALLABLE `{H : State.Trait} :
+    Global Instance AssociatedFunction_CALLABLE :
       Notation.DoubleColon Self "CALLABLE" := {
       Notation.double_colon := CALLABLE;
     }.
     
     Definition SELECTOR := Pure [ 11; 57; 111; 24 ].
     
-    Global Instance AssociatedFunction_SELECTOR `{H : State.Trait} :
+    Global Instance AssociatedFunction_SELECTOR :
       Notation.DoubleColon Self "SELECTOR" := {
       Notation.double_colon := SELECTOR;
     }.
     
     Definition PAYABLE := Pure false.
     
-    Global Instance AssociatedFunction_PAYABLE `{H : State.Trait} :
+    Global Instance AssociatedFunction_PAYABLE :
       Notation.DoubleColon Self "PAYABLE" := {
       Notation.double_colon := PAYABLE;
     }.
     
     Definition MUTATES := Pure true.
     
-    Global Instance AssociatedFunction_MUTATES `{H : State.Trait} :
+    Global Instance AssociatedFunction_MUTATES :
       Notation.DoubleColon Self "MUTATES" := {
       Notation.double_colon := MUTATES;
     }.
     
     Definition LABEL := Pure "transfer_from".
     
-    Global Instance AssociatedFunction_LABEL `{H : State.Trait} :
+    Global Instance AssociatedFunction_LABEL :
       Notation.DoubleColon Self "LABEL" := {
       Notation.double_colon := LABEL;
     }.
     
     Global Instance I :
         ink.reflect.dispatch.DispatchableMessageInfo.Trait Self := {
-      ink.reflect.dispatch.DispatchableMessageInfo.CALLABLE
-        `{H : State.Trait}
-        :=
-        CALLABLE;
-      ink.reflect.dispatch.DispatchableMessageInfo.MUTATES
-        `{H : State.Trait}
-        :=
-        MUTATES;
-      ink.reflect.dispatch.DispatchableMessageInfo.PAYABLE
-        `{H : State.Trait}
-        :=
-        PAYABLE;
-      ink.reflect.dispatch.DispatchableMessageInfo.SELECTOR
-        `{H : State.Trait}
-        :=
-        SELECTOR;
-      ink.reflect.dispatch.DispatchableMessageInfo.LABEL
-        `{H : State.Trait}
-        :=
-        LABEL;
+      ink.reflect.dispatch.DispatchableMessageInfo.CALLABLE := CALLABLE;
+      ink.reflect.dispatch.DispatchableMessageInfo.MUTATES := MUTATES;
+      ink.reflect.dispatch.DispatchableMessageInfo.PAYABLE := PAYABLE;
+      ink.reflect.dispatch.DispatchableMessageInfo.SELECTOR := SELECTOR;
+      ink.reflect.dispatch.DispatchableMessageInfo.LABEL := LABEL;
     }.
   End Impl_ink_reflect_dispatch_DispatchableMessageInfo_for_erc20_erc20_Erc20.
   
@@ -678,50 +570,37 @@ Module erc20.
   Module Impl_core_fmt_Debug_for_erc20_erc20_Erc20Ref.
     Definition Self := erc20.erc20.Erc20Ref.
     
-    Parameter debug_struct_field1_finish : core.fmt.Formatter -> string -> 
-      string -> ink_codegen_dispatch_info_ContractCallBuilder_Type -> 
-      M (H := H) core.fmt.Result.
-    
-    Global Instance Deb_debug_struct_field1_finish : Notation.DoubleColon
-      core.fmt.Formatter "debug_struct_field1_finish" := {
-      Notation.double_colon := debug_struct_field1_finish; }.
-    
     Definition fmt
-        `{H : State.Trait}
         (self : ref Self)
         (f : mut_ref core.fmt.Formatter)
-        : M (H := H) core.fmt.Result :=
+        : M core.fmt.Result :=
       core.fmt.Formatter::["debug_struct_field1_finish"]
         f
         "Erc20Ref"
         "inner"
         (addr_of (addr_of self.["inner"])).
     
-    Global Instance Method_fmt `{H : State.Trait} : Notation.Dot "fmt" := {
+    Global Instance Method_fmt : Notation.Dot "fmt" := {
       Notation.dot := fmt;
     }.
     
     Global Instance I : core.fmt.Debug.Trait Self := {
-      core.fmt.Debug.fmt `{H : State.Trait} := fmt;
+      core.fmt.Debug.fmt := fmt;
     }.
   End Impl_core_fmt_Debug_for_erc20_erc20_Erc20Ref.
   
   Module Impl_core_hash_Hash_for_erc20_erc20_Erc20Ref.
     Definition Self := erc20.erc20.Erc20Ref.
     
-    Definition hash
-        `{H : State.Trait}
-        (self : ref Self)
-        (state : mut_ref __H)
-        : M (H := H) unit :=
+    Definition hash (self : ref Self) (state : mut_ref __H) : M unit :=
       core.hash.Hash.hash (addr_of self.["inner"]) state.
     
-    Global Instance Method_hash `{H : State.Trait} : Notation.Dot "hash" := {
+    Global Instance Method_hash : Notation.Dot "hash" := {
       Notation.dot := hash;
     }.
     
     Global Instance I : core.hash.Hash.Trait Self := {
-      core.hash.Hash.hash `{H : State.Trait} := hash;
+      core.hash.Hash.hash := hash;
     }.
   End Impl_core_hash_Hash_for_erc20_erc20_Erc20Ref.
   
@@ -736,18 +615,17 @@ Module erc20.
     Definition Self := erc20.erc20.Erc20Ref.
     
     Definition eq
-        `{H : State.Trait}
         (self : ref Self)
         (other : ref erc20.erc20.Erc20Ref)
-        : M (H := H) bool :=
+        : M bool :=
       self.["inner"].["eq"] other.["inner"].
     
-    Global Instance Method_eq `{H : State.Trait} : Notation.Dot "eq" := {
+    Global Instance Method_eq : Notation.Dot "eq" := {
       Notation.dot := eq;
     }.
     
     Global Instance I : core.cmp.PartialEq.Trait Self := {
-      core.cmp.PartialEq.eq `{H : State.Trait} := eq;
+      core.cmp.PartialEq.eq := eq;
     }.
   End Impl_core_cmp_PartialEq_for_erc20_erc20_Erc20Ref.
   
@@ -761,14 +639,11 @@ Module erc20.
   Module Impl_core_cmp_Eq_for_erc20_erc20_Erc20Ref.
     Definition Self := erc20.erc20.Erc20Ref.
     
-    Definition assert_receiver_is_total_eq
-        `{H : State.Trait}
-        (self : ref Self)
-        : M (H := H) unit :=
+    Definition assert_receiver_is_total_eq (self : ref Self) : M unit :=
       let _ := tt in
       Pure tt.
     
-    Global Instance Method_assert_receiver_is_total_eq `{H : State.Trait} :
+    Global Instance Method_assert_receiver_is_total_eq :
       Notation.Dot "assert_receiver_is_total_eq" := {
       Notation.dot := assert_receiver_is_total_eq;
     }.
@@ -780,19 +655,16 @@ Module erc20.
   Module Impl_core_clone_Clone_for_erc20_erc20_Erc20Ref.
     Definition Self := erc20.erc20.Erc20Ref.
     
-    Definition clone
-        `{H : State.Trait}
-        (self : ref Self)
-        : M (H := H) erc20.erc20.Erc20Ref :=
+    Definition clone (self : ref Self) : M erc20.erc20.Erc20Ref :=
       let* α0 := core.clone.Clone.clone (addr_of self.["inner"]) in
       Pure {| erc20.erc20.Erc20Ref.inner := α0; |}.
     
-    Global Instance Method_clone `{H : State.Trait} : Notation.Dot "clone" := {
+    Global Instance Method_clone : Notation.Dot "clone" := {
       Notation.dot := clone;
     }.
     
     Global Instance I : core.clone.Clone.Trait Self := {
-      core.clone.Clone.clone `{H : State.Trait} := clone;
+      core.clone.Clone.clone := clone;
     }.
   End Impl_core_clone_Clone_for_erc20_erc20_Erc20Ref.
   
@@ -800,10 +672,9 @@ Module erc20.
     Definition Self := erc20.erc20.Erc20Ref.
     
     Definition new
-        `{H : State.Trait}
         (__ink_binding_0 : erc20.erc20.Balance)
         :
-          M (H := H)
+          M
             (ink_env.call.create_builder.CreateBuilder
               erc20.erc20.Environment
               Self
@@ -818,7 +689,7 @@ Module erc20.
               (ink_env.call.common.Unset ink_env.call.create_builder.state.Salt)
               (ink_env.call.common.Set
                 (ink_env.call.common.ReturnType Self))) :=
-      let* α0 := ink_env.call.create_builder.build_create tt in
+      let* α0 := ink_env.call.create_builder.build_create  in
       let* α1 :=
         ink_env.call.selector.Selector::["new"] [ 155; 174; 157; 94 ] in
       let* α2 := ink_env.call.execution_input.ExecutionInput::["new"] α1 in
@@ -826,15 +697,12 @@ Module erc20.
       let* α4 := α0.["exec_input"] α3 in
       α4.["returns"].
     
-    Global Instance AssociatedFunction_new `{H : State.Trait} :
+    Global Instance AssociatedFunction_new :
       Notation.DoubleColon Self "new" := {
       Notation.double_colon := new;
     }.
     
-    Definition total_supply
-        `{H : State.Trait}
-        (self : ref Self)
-        : M (H := H) erc20.erc20.Balance :=
+    Definition total_supply (self : ref Self) : M erc20.erc20.Balance :=
       let* α0 := self.["try_total_supply"] in
       α0.["unwrap_or_else"]
         (fun error =>
@@ -846,15 +714,13 @@ Module erc20.
               (addr_of [ α0 ]) in
           core.panicking.panic_fmt α1).
     
-    Global Instance Method_total_supply `{H : State.Trait} :
-      Notation.Dot "total_supply" := {
+    Global Instance Method_total_supply : Notation.Dot "total_supply" := {
       Notation.dot := total_supply;
     }.
     
     Definition try_total_supply
-        `{H : State.Trait}
         (self : ref Self)
-        : M (H := H) (ink_primitives.MessageResult erc20.erc20.Balance) :=
+        : M (ink_primitives.MessageResult erc20.erc20.Balance) :=
       let* α0 :=
         ink.codegen.trait_def.call_builder.TraitCallBuilder.call self in
       let* α1 := α0.["total_supply"] in
@@ -869,16 +735,15 @@ Module erc20.
               (addr_of [ α0 ]) in
           core.panicking.panic_fmt α1).
     
-    Global Instance Method_try_total_supply `{H : State.Trait} :
+    Global Instance Method_try_total_supply :
       Notation.Dot "try_total_supply" := {
       Notation.dot := try_total_supply;
     }.
     
     Definition balance_of
-        `{H : State.Trait}
         (self : ref Self)
         (owner : erc20.erc20.AccountId)
-        : M (H := H) erc20.erc20.Balance :=
+        : M erc20.erc20.Balance :=
       let* α0 := self.["try_balance_of"] owner in
       α0.["unwrap_or_else"]
         (fun error =>
@@ -890,16 +755,14 @@ Module erc20.
               (addr_of [ α0 ]) in
           core.panicking.panic_fmt α1).
     
-    Global Instance Method_balance_of `{H : State.Trait} :
-      Notation.Dot "balance_of" := {
+    Global Instance Method_balance_of : Notation.Dot "balance_of" := {
       Notation.dot := balance_of;
     }.
     
     Definition try_balance_of
-        `{H : State.Trait}
         (self : ref Self)
         (owner : erc20.erc20.AccountId)
-        : M (H := H) (ink_primitives.MessageResult erc20.erc20.Balance) :=
+        : M (ink_primitives.MessageResult erc20.erc20.Balance) :=
       let* α0 :=
         ink.codegen.trait_def.call_builder.TraitCallBuilder.call self in
       let* α1 := α0.["balance_of"] owner in
@@ -914,17 +777,15 @@ Module erc20.
               (addr_of [ α0 ]) in
           core.panicking.panic_fmt α1).
     
-    Global Instance Method_try_balance_of `{H : State.Trait} :
-      Notation.Dot "try_balance_of" := {
+    Global Instance Method_try_balance_of : Notation.Dot "try_balance_of" := {
       Notation.dot := try_balance_of;
     }.
     
     Definition allowance
-        `{H : State.Trait}
         (self : ref Self)
         (owner : erc20.erc20.AccountId)
         (spender : erc20.erc20.AccountId)
-        : M (H := H) erc20.erc20.Balance :=
+        : M erc20.erc20.Balance :=
       let* α0 := self.["try_allowance"] owner spender in
       α0.["unwrap_or_else"]
         (fun error =>
@@ -935,17 +796,15 @@ Module erc20.
               (addr_of [ α0 ]) in
           core.panicking.panic_fmt α1).
     
-    Global Instance Method_allowance `{H : State.Trait} :
-      Notation.Dot "allowance" := {
+    Global Instance Method_allowance : Notation.Dot "allowance" := {
       Notation.dot := allowance;
     }.
     
     Definition try_allowance
-        `{H : State.Trait}
         (self : ref Self)
         (owner : erc20.erc20.AccountId)
         (spender : erc20.erc20.AccountId)
-        : M (H := H) (ink_primitives.MessageResult erc20.erc20.Balance) :=
+        : M (ink_primitives.MessageResult erc20.erc20.Balance) :=
       let* α0 :=
         ink.codegen.trait_def.call_builder.TraitCallBuilder.call self in
       let* α1 := α0.["allowance"] owner spender in
@@ -959,17 +818,15 @@ Module erc20.
               (addr_of [ α0 ]) in
           core.panicking.panic_fmt α1).
     
-    Global Instance Method_try_allowance `{H : State.Trait} :
-      Notation.Dot "try_allowance" := {
+    Global Instance Method_try_allowance : Notation.Dot "try_allowance" := {
       Notation.dot := try_allowance;
     }.
     
     Definition transfer
-        `{H : State.Trait}
         (self : mut_ref Self)
         (to : erc20.erc20.AccountId)
         (value : erc20.erc20.Balance)
-        : M (H := H) (erc20.erc20.Result unit) :=
+        : M (erc20.erc20.Result unit) :=
       let* α0 := self.["try_transfer"] to value in
       α0.["unwrap_or_else"]
         (fun error =>
@@ -980,17 +837,15 @@ Module erc20.
               (addr_of [ α0 ]) in
           core.panicking.panic_fmt α1).
     
-    Global Instance Method_transfer `{H : State.Trait} :
-      Notation.Dot "transfer" := {
+    Global Instance Method_transfer : Notation.Dot "transfer" := {
       Notation.dot := transfer;
     }.
     
     Definition try_transfer
-        `{H : State.Trait}
         (self : mut_ref Self)
         (to : erc20.erc20.AccountId)
         (value : erc20.erc20.Balance)
-        : M (H := H) (ink_primitives.MessageResult (erc20.erc20.Result unit)) :=
+        : M (ink_primitives.MessageResult (erc20.erc20.Result unit)) :=
       let* α0 :=
         ink.codegen.trait_def.call_builder.TraitCallBuilder.call_mut self in
       let* α1 := α0.["transfer"] to value in
@@ -1004,17 +859,15 @@ Module erc20.
               (addr_of [ α0 ]) in
           core.panicking.panic_fmt α1).
     
-    Global Instance Method_try_transfer `{H : State.Trait} :
-      Notation.Dot "try_transfer" := {
+    Global Instance Method_try_transfer : Notation.Dot "try_transfer" := {
       Notation.dot := try_transfer;
     }.
     
     Definition approve
-        `{H : State.Trait}
         (self : mut_ref Self)
         (spender : erc20.erc20.AccountId)
         (value : erc20.erc20.Balance)
-        : M (H := H) (erc20.erc20.Result unit) :=
+        : M (erc20.erc20.Result unit) :=
       let* α0 := self.["try_approve"] spender value in
       α0.["unwrap_or_else"]
         (fun error =>
@@ -1025,17 +878,15 @@ Module erc20.
               (addr_of [ α0 ]) in
           core.panicking.panic_fmt α1).
     
-    Global Instance Method_approve `{H : State.Trait} :
-      Notation.Dot "approve" := {
+    Global Instance Method_approve : Notation.Dot "approve" := {
       Notation.dot := approve;
     }.
     
     Definition try_approve
-        `{H : State.Trait}
         (self : mut_ref Self)
         (spender : erc20.erc20.AccountId)
         (value : erc20.erc20.Balance)
-        : M (H := H) (ink_primitives.MessageResult (erc20.erc20.Result unit)) :=
+        : M (ink_primitives.MessageResult (erc20.erc20.Result unit)) :=
       let* α0 :=
         ink.codegen.trait_def.call_builder.TraitCallBuilder.call_mut self in
       let* α1 := α0.["approve"] spender value in
@@ -1049,18 +900,16 @@ Module erc20.
               (addr_of [ α0 ]) in
           core.panicking.panic_fmt α1).
     
-    Global Instance Method_try_approve `{H : State.Trait} :
-      Notation.Dot "try_approve" := {
+    Global Instance Method_try_approve : Notation.Dot "try_approve" := {
       Notation.dot := try_approve;
     }.
     
     Definition transfer_from
-        `{H : State.Trait}
         (self : mut_ref Self)
         (from : erc20.erc20.AccountId)
         (to : erc20.erc20.AccountId)
         (value : erc20.erc20.Balance)
-        : M (H := H) (erc20.erc20.Result unit) :=
+        : M (erc20.erc20.Result unit) :=
       let* α0 := self.["try_transfer_from"] from to value in
       α0.["unwrap_or_else"]
         (fun error =>
@@ -1072,18 +921,16 @@ Module erc20.
               (addr_of [ α0 ]) in
           core.panicking.panic_fmt α1).
     
-    Global Instance Method_transfer_from `{H : State.Trait} :
-      Notation.Dot "transfer_from" := {
+    Global Instance Method_transfer_from : Notation.Dot "transfer_from" := {
       Notation.dot := transfer_from;
     }.
     
     Definition try_transfer_from
-        `{H : State.Trait}
         (self : mut_ref Self)
         (from : erc20.erc20.AccountId)
         (to : erc20.erc20.AccountId)
         (value : erc20.erc20.Balance)
-        : M (H := H) (ink_primitives.MessageResult (erc20.erc20.Result unit)) :=
+        : M (ink_primitives.MessageResult (erc20.erc20.Result unit)) :=
       let* α0 :=
         ink.codegen.trait_def.call_builder.TraitCallBuilder.call_mut self in
       let* α1 := α0.["transfer_from"] from to value in
@@ -1098,7 +945,7 @@ Module erc20.
               (addr_of [ α0 ]) in
           core.panicking.panic_fmt α1).
     
-    Global Instance Method_try_transfer_from `{H : State.Trait} :
+    Global Instance Method_try_transfer_from :
       Notation.Dot "try_transfer_from" := {
       Notation.dot := try_transfer_from;
     }.
@@ -1108,15 +955,12 @@ Module erc20.
     Impl_ink_env_call_create_builder_FromAccountId_for_erc20_erc20_Erc20Ref.
     Definition Self := erc20.erc20.Erc20Ref.
     
-    Definition from_account_id
-        `{H : State.Trait}
-        (account_id : erc20.erc20.AccountId)
-        : M (H := H) Self :=
+    Definition from_account_id (account_id : erc20.erc20.AccountId) : M Self :=
       let* α0 :=
         ink_env.call.create_builder.FromAccountId.from_account_id account_id in
       Pure {| Self.inner := α0; |}.
     
-    Global Instance AssociatedFunction_from_account_id `{H : State.Trait} :
+    Global Instance AssociatedFunction_from_account_id :
       Notation.DoubleColon Self "from_account_id" := {
       Notation.double_colon := from_account_id;
     }.
@@ -1126,7 +970,6 @@ Module erc20.
           Self
           (T := erc20.erc20.Environment) := {
       ink_env.call.create_builder.FromAccountId.from_account_id
-        `{H : State.Trait}
         :=
         from_account_id;
     }.
@@ -1135,14 +978,10 @@ Module erc20.
   Module Impl_ink_contract_ref_ToAccountId_for_erc20_erc20_Erc20Ref.
     Definition Self := erc20.erc20.Erc20Ref.
     
-    Definition to_account_id
-        `{H : State.Trait}
-        (self : ref Self)
-        : M (H := H) erc20.erc20.AccountId :=
+    Definition to_account_id (self : ref Self) : M erc20.erc20.AccountId :=
       ink.contract_ref.ToAccountId.to_account_id (addr_of self.["inner"]).
     
-    Global Instance Method_to_account_id `{H : State.Trait} :
-      Notation.Dot "to_account_id" := {
+    Global Instance Method_to_account_id : Notation.Dot "to_account_id" := {
       Notation.dot := to_account_id;
     }.
     
@@ -1150,30 +989,23 @@ Module erc20.
         ink.contract_ref.ToAccountId.Trait
           Self
           (T := erc20.erc20.Environment) := {
-      ink.contract_ref.ToAccountId.to_account_id
-        `{H : State.Trait}
-        :=
-        to_account_id;
+      ink.contract_ref.ToAccountId.to_account_id := to_account_id;
     }.
   End Impl_ink_contract_ref_ToAccountId_for_erc20_erc20_Erc20Ref.
   
   Module Impl_core_convert_AsRef_for_erc20_erc20_Erc20Ref.
     Definition Self := erc20.erc20.Erc20Ref.
     
-    Definition as_ref
-        `{H : State.Trait}
-        (self : ref Self)
-        : M (H := H) (ref erc20.erc20.AccountId) :=
+    Definition as_ref (self : ref Self) : M (ref erc20.erc20.AccountId) :=
       core.convert.AsRef.as_ref (addr_of self.["inner"]).
     
-    Global Instance Method_as_ref `{H : State.Trait} :
-      Notation.Dot "as_ref" := {
+    Global Instance Method_as_ref : Notation.Dot "as_ref" := {
       Notation.dot := as_ref;
     }.
     
     Global Instance I :
         core.convert.AsRef.Trait Self (T := erc20.erc20.AccountId) := {
-      core.convert.AsRef.as_ref `{H : State.Trait} := as_ref;
+      core.convert.AsRef.as_ref := as_ref;
     }.
   End Impl_core_convert_AsRef_for_erc20_erc20_Erc20Ref.
   
@@ -1181,19 +1013,17 @@ Module erc20.
     Definition Self := erc20.erc20.Erc20Ref.
     
     Definition as_mut
-        `{H : State.Trait}
         (self : mut_ref Self)
-        : M (H := H) (mut_ref erc20.erc20.AccountId) :=
+        : M (mut_ref erc20.erc20.AccountId) :=
       core.convert.AsMut.as_mut (addr_of self.["inner"]).
     
-    Global Instance Method_as_mut `{H : State.Trait} :
-      Notation.Dot "as_mut" := {
+    Global Instance Method_as_mut : Notation.Dot "as_mut" := {
       Notation.dot := as_mut;
     }.
     
     Global Instance I :
         core.convert.AsMut.Trait Self (T := erc20.erc20.AccountId) := {
-      core.convert.AsMut.as_mut `{H : State.Trait} := as_mut;
+      core.convert.AsMut.as_mut := as_mut;
     }.
   End Impl_core_convert_AsMut_for_erc20_erc20_Erc20Ref.
   
@@ -1208,10 +1038,9 @@ Module erc20.
     Definition Self := erc20.erc20.Error.
     
     Definition fmt
-        `{H : State.Trait}
         (self : ref Self)
         (f : mut_ref core.fmt.Formatter)
-        : M (H := H) core.fmt.Result :=
+        : M core.fmt.Result :=
       let* α0 :=
         match self with
         | erc20.erc20.Error.InsufficientBalance => Pure "InsufficientBalance"
@@ -1220,12 +1049,12 @@ Module erc20.
         end in
       core.fmt.Formatter::["write_str"] f α0.
     
-    Global Instance Method_fmt `{H : State.Trait} : Notation.Dot "fmt" := {
+    Global Instance Method_fmt : Notation.Dot "fmt" := {
       Notation.dot := fmt;
     }.
     
     Global Instance I : core.fmt.Debug.Trait Self := {
-      core.fmt.Debug.fmt `{H : State.Trait} := fmt;
+      core.fmt.Debug.fmt := fmt;
     }.
   End Impl_core_fmt_Debug_for_erc20_erc20_Error.
   
@@ -1239,21 +1068,17 @@ Module erc20.
   Module Impl_core_cmp_PartialEq_for_erc20_erc20_Error.
     Definition Self := erc20.erc20.Error.
     
-    Definition eq
-        `{H : State.Trait}
-        (self : ref Self)
-        (other : ref erc20.erc20.Error)
-        : M (H := H) bool :=
+    Definition eq (self : ref Self) (other : ref erc20.erc20.Error) : M bool :=
       let* __self_tag := core.intrinsics.discriminant_value self in
       let* __arg1_tag := core.intrinsics.discriminant_value other in
       __self_tag.["eq"] __arg1_tag.
     
-    Global Instance Method_eq `{H : State.Trait} : Notation.Dot "eq" := {
+    Global Instance Method_eq : Notation.Dot "eq" := {
       Notation.dot := eq;
     }.
     
     Global Instance I : core.cmp.PartialEq.Trait Self := {
-      core.cmp.PartialEq.eq `{H : State.Trait} := eq;
+      core.cmp.PartialEq.eq := eq;
     }.
   End Impl_core_cmp_PartialEq_for_erc20_erc20_Error.
   
@@ -1267,13 +1092,10 @@ Module erc20.
   Module Impl_core_cmp_Eq_for_erc20_erc20_Error.
     Definition Self := erc20.erc20.Error.
     
-    Definition assert_receiver_is_total_eq
-        `{H : State.Trait}
-        (self : ref Self)
-        : M (H := H) unit :=
+    Definition assert_receiver_is_total_eq (self : ref Self) : M unit :=
       Pure tt.
     
-    Global Instance Method_assert_receiver_is_total_eq `{H : State.Trait} :
+    Global Instance Method_assert_receiver_is_total_eq :
       Notation.Dot "assert_receiver_is_total_eq" := {
       Notation.dot := assert_receiver_is_total_eq;
     }.
@@ -1308,7 +1130,7 @@ Definition BlockNumber : Set := ink_env.types.Environment.BlockNumber.
 
 Definition ChainExtension : Set := ink_env.types.Environment.ChainExtension.
 
-Definition MAX_EVENT_TOPICS `{H : State.Trait} : usize :=
+Definition MAX_EVENT_TOPICS : usize :=
   run (Pure ink_env.types.Environment.MAX_EVENT_TOPICS).
 
 Module Check.
@@ -1384,13 +1206,12 @@ Module Impl_ink_storage_traits_storage_StorageKey_for_erc20_erc20_Erc20.
   
   Definition KEY := Pure ink_storage_traits.storage.StorageKey.KEY.
   
-  Global Instance AssociatedFunction_KEY `{H : State.Trait} :
-    Notation.DoubleColon Self "KEY" := {
+  Global Instance AssociatedFunction_KEY : Notation.DoubleColon Self "KEY" := {
     Notation.double_colon := KEY;
   }.
   
   Global Instance I : ink_storage_traits.storage.StorageKey.Trait Self := {
-    ink_storage_traits.storage.StorageKey.KEY `{H : State.Trait} := KEY;
+    ink_storage_traits.storage.StorageKey.KEY := KEY;
   }.
 End Impl_ink_storage_traits_storage_StorageKey_for_erc20_erc20_Erc20.
 
@@ -1398,9 +1219,8 @@ Module Impl_ink_storage_traits_storage_Storable_for_erc20_erc20_Erc20.
   Definition Self := erc20.erc20.Erc20.
   
   Definition decode
-      `{H : State.Trait}
       (__input : mut_ref __ink_I)
-      : M (H := H) (core.result.Result Self parity_scale_codec.error.Error) :=
+      : M (core.result.Result Self parity_scale_codec.error.Error) :=
     let* α0 := ink_storage_traits.storage.Storable.decode __input in
     let* α1 := LangItem α0 in
     let* α2 :=
@@ -1436,16 +1256,12 @@ Module Impl_ink_storage_traits_storage_Storable_for_erc20_erc20_Erc20.
           erc20.erc20.Erc20.allowances := α8;
         |}).
   
-  Global Instance AssociatedFunction_decode `{H : State.Trait} :
+  Global Instance AssociatedFunction_decode :
     Notation.DoubleColon Self "decode" := {
     Notation.double_colon := decode;
   }.
   
-  Definition encode
-      `{H : State.Trait}
-      (self : ref Self)
-      (__dest : mut_ref __ink_O)
-      : M (H := H) unit :=
+  Definition encode (self : ref Self) (__dest : mut_ref __ink_O) : M unit :=
     match self with
     |
         {|
@@ -1466,13 +1282,13 @@ Module Impl_ink_storage_traits_storage_Storable_for_erc20_erc20_Erc20.
       Pure tt
     end.
   
-  Global Instance Method_encode `{H : State.Trait} : Notation.Dot "encode" := {
+  Global Instance Method_encode : Notation.Dot "encode" := {
     Notation.dot := encode;
   }.
   
   Global Instance I : ink_storage_traits.storage.Storable.Trait Self := {
-    ink_storage_traits.storage.Storable.encode `{H : State.Trait} := encode;
-    ink_storage_traits.storage.Storable.decode `{H : State.Trait} := decode;
+    ink_storage_traits.storage.Storable.encode := encode;
+    ink_storage_traits.storage.Storable.decode := decode;
   }.
 End Impl_ink_storage_traits_storage_Storable_for_erc20_erc20_Erc20.
 
@@ -1481,17 +1297,14 @@ Module Impl_scale_info_TypeInfo_for_erc20_erc20_Erc20.
   
   Definition Identity : Set := Self.
   
-  Definition type_info
-      `{H : State.Trait}
-      (_ : unit)
-      : M (H := H) scale_info.ty.Type :=
-    let* α0 := scale_info.ty.Type::["builder"] tt in
+  Definition type_info  : M scale_info.ty.Type :=
+    let* α0 := scale_info.ty.Type::["builder"]  in
     let* α1 := scale_info.ty.path.Path::["new"] "Erc20" "erc20::erc20" in
     let* α2 := α0.["path"] α1 in
-    let* α3 := alloc.vec.Vec::["new"] tt in
+    let* α3 := alloc.vec.Vec::["new"]  in
     let* α4 := α2.["type_params"] α3 in
     let* α5 := α4.["docs"] (addr_of [ "A simple ERC-20 contract." ]) in
-    let* α6 := scale_info.build.Fields::["named"] tt in
+    let* α6 := scale_info.build.Fields::["named"]  in
     let* α7 :=
       α6.["field"]
         (fun f =>
@@ -1532,13 +1345,13 @@ AutoStorableHint<::ink::storage::traits::ManualKey<639884519u32, ()
               ])) in
     α5.["composite"] α9.
   
-  Global Instance AssociatedFunction_type_info `{H : State.Trait} :
+  Global Instance AssociatedFunction_type_info :
     Notation.DoubleColon Self "type_info" := {
     Notation.double_colon := type_info;
   }.
   
   Global Instance I : scale_info.TypeInfo.Trait Self := {
-    scale_info.TypeInfo.type_info `{H : State.Trait} := type_info;
+    scale_info.TypeInfo.type_info := type_info;
   }.
 End Impl_scale_info_TypeInfo_for_erc20_erc20_Erc20.
 
@@ -1546,9 +1359,8 @@ Module Impl_ink_storage_traits_layout_StorageLayout_for_erc20_erc20_Erc20.
   Definition Self := erc20.erc20.Erc20.
   
   Definition layout
-      `{H : State.Trait}
       (__key : ref ink_primitives.key.Key)
-      : M (H := H) ink_metadata.layout.Layout :=
+      : M ink_metadata.layout.Layout :=
     let* α0 := ink_storage_traits.layout.StorageLayout.layout __key in
     let* α1 := ink_metadata.layout.FieldLayout::["new"] "total_supply" α0 in
     let* α2 := ink_storage_traits.layout.StorageLayout.layout __key in
@@ -1559,26 +1371,23 @@ Module Impl_ink_storage_traits_layout_StorageLayout_for_erc20_erc20_Erc20.
       ink_metadata.layout.StructLayout::["new"] "Erc20" [ α1; α3; α5 ] in
     Pure (ink_metadata.layout.Layout.Struct α6).
   
-  Global Instance AssociatedFunction_layout `{H : State.Trait} :
+  Global Instance AssociatedFunction_layout :
     Notation.DoubleColon Self "layout" := {
     Notation.double_colon := layout;
   }.
   
   Global Instance I : ink_storage_traits.layout.StorageLayout.Trait Self := {
-    ink_storage_traits.layout.StorageLayout.layout `{H : State.Trait} := layout;
+    ink_storage_traits.layout.StorageLayout.layout := layout;
   }.
 End Impl_ink_storage_traits_layout_StorageLayout_for_erc20_erc20_Erc20.
 
 Module Impl_core_default_Default_for_erc20_erc20_Erc20.
   Definition Self := erc20.erc20.Erc20.
   
-  Definition default
-      `{H : State.Trait}
-      (_ : unit)
-      : M (H := H) erc20.erc20.Erc20 :=
-    let* α0 := core.default.Default.default tt in
-    let* α1 := core.default.Default.default tt in
-    let* α2 := core.default.Default.default tt in
+  Definition default  : M erc20.erc20.Erc20 :=
+    let* α0 := core.default.Default.default  in
+    let* α1 := core.default.Default.default  in
+    let* α2 := core.default.Default.default  in
     Pure
       {|
         erc20.erc20.Erc20.total_supply := α0;
@@ -1586,13 +1395,13 @@ Module Impl_core_default_Default_for_erc20_erc20_Erc20.
         erc20.erc20.Erc20.allowances := α2;
       |}.
   
-  Global Instance AssociatedFunction_default `{H : State.Trait} :
+  Global Instance AssociatedFunction_default :
     Notation.DoubleColon Self "default" := {
     Notation.double_colon := default;
   }.
   
   Global Instance I : core.default.Default.Trait Self := {
-    core.default.Default.default `{H : State.Trait} := default;
+    core.default.Default.default := default;
   }.
 End Impl_core_default_Default_for_erc20_erc20_Erc20.
 
@@ -1601,13 +1410,13 @@ Module Impl_ink_reflect_contract_ContractName_for_erc20_erc20_Erc20.
   
   Definition NAME := Pure "Erc20".
   
-  Global Instance AssociatedFunction_NAME `{H : State.Trait} :
+  Global Instance AssociatedFunction_NAME :
     Notation.DoubleColon Self "NAME" := {
     Notation.double_colon := NAME;
   }.
   
   Global Instance I : ink.reflect.contract.ContractName.Trait Self := {
-    ink.reflect.contract.ContractName.NAME `{H : State.Trait} := NAME;
+    ink.reflect.contract.ContractName.NAME := NAME;
   }.
 End Impl_ink_reflect_contract_ContractName_for_erc20_erc20_Erc20.
 
@@ -1617,18 +1426,15 @@ Module Impl_ink_codegen_env_Env_for_StaticRef_erc20_erc20_Erc20.
   Definition EnvAccess : Set :=
     ink.env_access.EnvAccess ink_env.contract.ContractEnv.Env.
   
-  Definition env
-      `{H : State.Trait}
-      (self : Self)
-      : M (H := H) ImplSelf.EnvAccess :=
-    core.default.Default.default tt.
+  Definition env (self : Self) : M ImplSelf.EnvAccess :=
+    core.default.Default.default .
   
-  Global Instance Method_env `{H : State.Trait} : Notation.Dot "env" := {
+  Global Instance Method_env : Notation.Dot "env" := {
     Notation.dot := env;
   }.
   
   Global Instance I : ink.codegen.env.Env.Trait Self := {
-    ink.codegen.env.Env.env `{H : State.Trait} := env;
+    ink.codegen.env.Env.env := env;
   }.
 End Impl_ink_codegen_env_Env_for_StaticRef_erc20_erc20_Erc20.
 
@@ -1638,19 +1444,14 @@ Module Impl_ink_codegen_env_StaticEnv_for_erc20_erc20_Erc20.
   Definition EnvAccess : Set :=
     ink.env_access.EnvAccess ink_env.contract.ContractEnv.Env.
   
-  Definition env
-      `{H : State.Trait}
-      (_ : unit)
-      : M (H := H) ImplSelf.EnvAccess :=
-    core.default.Default.default tt.
+  Definition env  : M ImplSelf.EnvAccess := core.default.Default.default .
   
-  Global Instance AssociatedFunction_env `{H : State.Trait} :
-    Notation.DoubleColon Self "env" := {
+  Global Instance AssociatedFunction_env : Notation.DoubleColon Self "env" := {
     Notation.double_colon := env;
   }.
   
   Global Instance I : ink.codegen.env.StaticEnv.Trait Self := {
-    ink.codegen.env.StaticEnv.env `{H : State.Trait} := env;
+    ink.codegen.env.StaticEnv.env := env;
   }.
 End Impl_ink_codegen_env_StaticEnv_for_erc20_erc20_Erc20.
 
@@ -1658,27 +1459,19 @@ Module
   Impl_ink_codegen_event_emit_EmitEvent_for_ink_env_access_EnvAccess_erc20_erc20_Environment.
   Definition Self := ink.env_access.EnvAccess erc20.erc20.Environment.
   
-  Definition emit_event
-      `{H : State.Trait}
-      (self : Self)
-      (event : E)
-      : M (H := H) unit :=
+  Definition emit_event (self : Self) (event : E) : M unit :=
     let* _ :=
       let* α0 := event.["into"] in
       ink_env.api.emit_event α0 in
     Pure tt.
   
-  Global Instance Method_emit_event `{H : State.Trait} :
-    Notation.Dot "emit_event" := {
+  Global Instance Method_emit_event : Notation.Dot "emit_event" := {
     Notation.dot := emit_event;
   }.
   
   Global Instance I :
       ink.codegen.event.emit.EmitEvent.Trait Self (C := erc20.erc20.Erc20) := {
-    ink.codegen.event.emit.EmitEvent.emit_event
-      `{H : State.Trait}
-      :=
-      emit_event;
+    ink.codegen.event.emit.EmitEvent.emit_event := emit_event;
   }.
 End
   Impl_ink_codegen_event_emit_EmitEvent_for_ink_env_access_EnvAccess_erc20_erc20_Environment.
@@ -1694,10 +1487,9 @@ Module Impl_parity_scale_codec_codec_Encode_for_erc20_erc20___ink_EventBase.
   Definition Self := erc20.erc20.__ink_EventBase.
   
   Definition encode_to
-      `{H : State.Trait}
       (self : ref Self)
       (__codec_dest_edqy : mut_ref __CodecOutputEdqy)
-      : M (H := H) unit :=
+      : M unit :=
     let* α0 := self.["deref"] in
     match α0 with
     | erc20.erc20.__ink_EventBase.Transfer aa =>
@@ -1715,8 +1507,7 @@ Module Impl_parity_scale_codec_codec_Encode_for_erc20_erc20___ink_EventBase.
     | _ => Pure tt
     end.
   
-  Global Instance Method_encode_to `{H : State.Trait} :
-    Notation.Dot "encode_to" := {
+  Global Instance Method_encode_to : Notation.Dot "encode_to" := {
     Notation.dot := encode_to;
   }.
   
@@ -1737,9 +1528,8 @@ Module Impl_parity_scale_codec_codec_Decode_for_erc20_erc20___ink_EventBase.
   Definition Self := erc20.erc20.__ink_EventBase.
   
   Definition decode
-      `{H : State.Trait}
       (__codec_input_edqy : mut_ref __CodecInputEdqy)
-      : M (H := H) (core.result.Result Self parity_scale_codec.error.Error) :=
+      : M (core.result.Result Self parity_scale_codec.error.Error) :=
     let* α0 := __codec_input_edqy.["read_byte"] in
     let* α1 :=
       α0.["map_err"]
@@ -1774,7 +1564,7 @@ Module Impl_parity_scale_codec_codec_Decode_for_erc20_erc20___ink_EventBase.
               Pure
                 (core.result.Result.Ok
                   (erc20.erc20.__ink_EventBase.Transfer α0)))
-            tt in
+             in
         Return α0 in
       Pure tt
     | __codec_x_edqy =>
@@ -1796,7 +1586,7 @@ Module Impl_parity_scale_codec_codec_Decode_for_erc20_erc20___ink_EventBase.
               Pure
                 (core.result.Result.Ok
                   (erc20.erc20.__ink_EventBase.Approval α0)))
-            tt in
+             in
         Return α0 in
       Pure tt
     | _ =>
@@ -1807,18 +1597,18 @@ Module Impl_parity_scale_codec_codec_Decode_for_erc20_erc20___ink_EventBase.
                 core.convert.Into.into
                   "Could not decode `__ink_EventBase`, variant doesn't exist" in
               Pure (core.result.Result.Err α0))
-            tt in
+             in
         Return α0 in
       Pure tt
     end.
   
-  Global Instance AssociatedFunction_decode `{H : State.Trait} :
+  Global Instance AssociatedFunction_decode :
     Notation.DoubleColon Self "decode" := {
     Notation.double_colon := decode;
   }.
   
   Global Instance I : parity_scale_codec.codec.Decode.Trait Self := {
-    parity_scale_codec.codec.Decode.decode `{H : State.Trait} := decode;
+    parity_scale_codec.codec.Decode.decode := decode;
   }.
 End Impl_parity_scale_codec_codec_Decode_for_erc20_erc20___ink_EventBase.
 
@@ -1834,40 +1624,34 @@ End Impl_ink_reflect_event_ContractEventBase_for_erc20_erc20_Erc20.
 Module Impl_core_convert_From_for_erc20_erc20___ink_EventBase.
   Definition Self := erc20.erc20.__ink_EventBase.
   
-  Definition from
-      `{H : State.Trait}
-      (event : erc20.erc20.Transfer)
-      : M (H := H) Self :=
+  Definition from (event : erc20.erc20.Transfer) : M Self :=
     Self::["Transfer"] event.
   
-  Global Instance AssociatedFunction_from `{H : State.Trait} :
+  Global Instance AssociatedFunction_from :
     Notation.DoubleColon Self "from" := {
     Notation.double_colon := from;
   }.
   
   Global Instance I :
       core.convert.From.Trait Self (T := erc20.erc20.Transfer) := {
-    core.convert.From.from `{H : State.Trait} := from;
+    core.convert.From.from := from;
   }.
 End Impl_core_convert_From_for_erc20_erc20___ink_EventBase.
 
 Module Impl_core_convert_From_for_erc20_erc20___ink_EventBase.
   Definition Self := erc20.erc20.__ink_EventBase.
   
-  Definition from
-      `{H : State.Trait}
-      (event : erc20.erc20.Approval)
-      : M (H := H) Self :=
+  Definition from (event : erc20.erc20.Approval) : M Self :=
     Self::["Approval"] event.
   
-  Global Instance AssociatedFunction_from `{H : State.Trait} :
+  Global Instance AssociatedFunction_from :
     Notation.DoubleColon Self "from" := {
     Notation.double_colon := from;
   }.
   
   Global Instance I :
       core.convert.From.Trait Self (T := erc20.erc20.Approval) := {
-    core.convert.From.from `{H : State.Trait} := from;
+    core.convert.From.from := from;
   }.
 End Impl_core_convert_From_for_erc20_erc20___ink_EventBase.
 
@@ -1883,13 +1667,13 @@ Module
   
   Definition AMOUNT := Pure 0.
   
-  Global Instance AssociatedFunction_AMOUNT `{H : State.Trait} :
+  Global Instance AssociatedFunction_AMOUNT :
     Notation.DoubleColon Self "AMOUNT" := {
     Notation.double_colon := AMOUNT;
   }.
   
   Global Instance I : ink_env.topics.EventTopicsAmount.Trait Self := {
-    ink_env.topics.EventTopicsAmount.AMOUNT `{H : State.Trait} := AMOUNT;
+    ink_env.topics.EventTopicsAmount.AMOUNT := AMOUNT;
   }.
 End
   Impl_ink_env_topics_EventTopicsAmount_for_erc20_erc20_____ink_UndefinedAmountOfTopics.
@@ -1901,10 +1685,9 @@ Module Impl_ink_env_topics_Topics_for_erc20_erc20___ink_EventBase.
     erc20.erc20._.__ink_UndefinedAmountOfTopics.
   
   Definition topics
-      `{H : State.Trait}
       (self : ref Self)
       (builder : ink_env.topics.TopicsBuilder ink_env.topics.state.Uninit E B)
-      : M (H := H) ink_env.topics.TopicsBuilderBackend.Output :=
+      : M ink_env.topics.TopicsBuilderBackend.Output :=
     match self with
     | ImplSelf.Transfer.Build_t event =>
       ink_env.topics.Topics.topics event builder
@@ -1916,12 +1699,12 @@ Module Impl_ink_env_topics_Topics_for_erc20_erc20___ink_EventBase.
       core.panicking.panic_fmt α0
     end.
   
-  Global Instance Method_topics `{H : State.Trait} : Notation.Dot "topics" := {
+  Global Instance Method_topics : Notation.Dot "topics" := {
     Notation.dot := topics;
   }.
   
   Global Instance I : ink_env.topics.Topics.Trait Self := {
-    ink_env.topics.Topics.topics `{H : State.Trait} := topics;
+    ink_env.topics.Topics.topics := topics;
   }.
 End Impl_ink_env_topics_Topics_for_erc20_erc20___ink_EventBase.
 
@@ -1966,10 +1749,9 @@ Module Impl_parity_scale_codec_codec_Encode_for_erc20_erc20_Transfer.
   Definition Self := erc20.erc20.Transfer.
   
   Definition encode_to
-      `{H : State.Trait}
       (self : ref Self)
       (__codec_dest_edqy : mut_ref __CodecOutputEdqy)
-      : M (H := H) unit :=
+      : M unit :=
     let* _ :=
       parity_scale_codec.codec.Encode.encode_to
         (addr_of self.["from"])
@@ -1984,8 +1766,7 @@ Module Impl_parity_scale_codec_codec_Encode_for_erc20_erc20_Transfer.
         __codec_dest_edqy in
     Pure tt.
   
-  Global Instance Method_encode_to `{H : State.Trait} :
-    Notation.Dot "encode_to" := {
+  Global Instance Method_encode_to : Notation.Dot "encode_to" := {
     Notation.dot := encode_to;
   }.
   
@@ -2004,9 +1785,8 @@ Module Impl_parity_scale_codec_codec_Decode_for_erc20_erc20_Transfer.
   Definition Self := erc20.erc20.Transfer.
   
   Definition decode
-      `{H : State.Trait}
       (__codec_input_edqy : mut_ref __CodecInputEdqy)
-      : M (H := H) (core.result.Result Self parity_scale_codec.error.Error) :=
+      : M (core.result.Result Self parity_scale_codec.error.Error) :=
     let* __codec_res_edqy :=
       parity_scale_codec.codec.Decode.decode __codec_input_edqy in
     let* α0 :=
@@ -2042,13 +1822,13 @@ Module Impl_parity_scale_codec_codec_Decode_for_erc20_erc20_Transfer.
           erc20.erc20.Transfer.value := α2;
         |}).
   
-  Global Instance AssociatedFunction_decode `{H : State.Trait} :
+  Global Instance AssociatedFunction_decode :
     Notation.DoubleColon Self "decode" := {
     Notation.double_colon := decode;
   }.
   
   Global Instance I : parity_scale_codec.codec.Decode.Trait Self := {
-    parity_scale_codec.codec.Decode.decode `{H : State.Trait} := decode;
+    parity_scale_codec.codec.Decode.decode := decode;
   }.
 End Impl_parity_scale_codec_codec_Decode_for_erc20_erc20_Transfer.
 
@@ -2075,10 +1855,9 @@ Module Impl_parity_scale_codec_codec_Encode_for_erc20_erc20_Approval.
   Definition Self := erc20.erc20.Approval.
   
   Definition encode_to
-      `{H : State.Trait}
       (self : ref Self)
       (__codec_dest_edqy : mut_ref __CodecOutputEdqy)
-      : M (H := H) unit :=
+      : M unit :=
     let* _ :=
       parity_scale_codec.codec.Encode.encode_to
         (addr_of self.["owner"])
@@ -2093,8 +1872,7 @@ Module Impl_parity_scale_codec_codec_Encode_for_erc20_erc20_Approval.
         __codec_dest_edqy in
     Pure tt.
   
-  Global Instance Method_encode_to `{H : State.Trait} :
-    Notation.Dot "encode_to" := {
+  Global Instance Method_encode_to : Notation.Dot "encode_to" := {
     Notation.dot := encode_to;
   }.
   
@@ -2113,9 +1891,8 @@ Module Impl_parity_scale_codec_codec_Decode_for_erc20_erc20_Approval.
   Definition Self := erc20.erc20.Approval.
   
   Definition decode
-      `{H : State.Trait}
       (__codec_input_edqy : mut_ref __CodecInputEdqy)
-      : M (H := H) (core.result.Result Self parity_scale_codec.error.Error) :=
+      : M (core.result.Result Self parity_scale_codec.error.Error) :=
     let* __codec_res_edqy :=
       parity_scale_codec.codec.Decode.decode __codec_input_edqy in
     let* α0 :=
@@ -2151,13 +1928,13 @@ Module Impl_parity_scale_codec_codec_Decode_for_erc20_erc20_Approval.
           erc20.erc20.Approval.value := α2;
         |}).
   
-  Global Instance AssociatedFunction_decode `{H : State.Trait} :
+  Global Instance AssociatedFunction_decode :
     Notation.DoubleColon Self "decode" := {
     Notation.double_colon := decode;
   }.
   
   Global Instance I : parity_scale_codec.codec.Decode.Trait Self := {
-    parity_scale_codec.codec.Decode.decode `{H : State.Trait} := decode;
+    parity_scale_codec.codec.Decode.decode := decode;
   }.
 End Impl_parity_scale_codec_codec_Decode_for_erc20_erc20_Approval.
 
@@ -2168,10 +1945,9 @@ Module Impl_ink_env_topics_Topics_for_erc20_erc20_Transfer.
     list ink_env.topics.state.HasRemainingTopics.
   
   Definition topics
-      `{H : State.Trait}
       (self : ref Self)
       (builder : ink_env.topics.TopicsBuilder ink_env.topics.state.Uninit E B)
-      : M (H := H) ink_env.topics.TopicsBuilderBackend.Output :=
+      : M ink_env.topics.TopicsBuilderBackend.Output :=
     let* α0 := builder.["build"] in
     let* α1 :=
       α0.["push_topic"]
@@ -2199,12 +1975,12 @@ Module Impl_ink_env_topics_Topics_for_erc20_erc20_Transfer.
           |}) in
     α3.["finish"].
   
-  Global Instance Method_topics `{H : State.Trait} : Notation.Dot "topics" := {
+  Global Instance Method_topics : Notation.Dot "topics" := {
     Notation.dot := topics;
   }.
   
   Global Instance I : ink_env.topics.Topics.Trait Self := {
-    ink_env.topics.Topics.topics `{H : State.Trait} := topics;
+    ink_env.topics.Topics.topics := topics;
   }.
 End Impl_ink_env_topics_Topics_for_erc20_erc20_Transfer.
 
@@ -2215,10 +1991,9 @@ Module Impl_ink_env_topics_Topics_for_erc20_erc20_Approval.
     list ink_env.topics.state.HasRemainingTopics.
   
   Definition topics
-      `{H : State.Trait}
       (self : ref Self)
       (builder : ink_env.topics.TopicsBuilder ink_env.topics.state.Uninit E B)
-      : M (H := H) ink_env.topics.TopicsBuilderBackend.Output :=
+      : M ink_env.topics.TopicsBuilderBackend.Output :=
     let* α0 := builder.["build"] in
     let* α1 :=
       α0.["push_topic"]
@@ -2246,12 +2021,12 @@ Module Impl_ink_env_topics_Topics_for_erc20_erc20_Approval.
           |}) in
     α3.["finish"].
   
-  Global Instance Method_topics `{H : State.Trait} : Notation.Dot "topics" := {
+  Global Instance Method_topics : Notation.Dot "topics" := {
     Notation.dot := topics;
   }.
   
   Global Instance I : ink_env.topics.Topics.Trait Self := {
-    ink_env.topics.Topics.topics `{H : State.Trait} := topics;
+    ink_env.topics.Topics.topics := topics;
   }.
 End Impl_ink_env_topics_Topics_for_erc20_erc20_Approval.
 
@@ -2269,7 +2044,7 @@ Module
   
   Definition IS_RESULT := Pure ink.reflect.dispatch.ConstructorOutput.IS_RESULT.
   
-  Global Instance AssociatedFunction_IS_RESULT `{H : State.Trait} :
+  Global Instance AssociatedFunction_IS_RESULT :
     Notation.DoubleColon Self "IS_RESULT" := {
     Notation.double_colon := IS_RESULT;
   }.
@@ -2278,54 +2053,39 @@ Module
     CALLABLE := Pure
       (fun __ink_binding_0 => erc20.erc20.Erc20::["new"] __ink_binding_0).
   
-  Global Instance AssociatedFunction_CALLABLE `{H : State.Trait} :
+  Global Instance AssociatedFunction_CALLABLE :
     Notation.DoubleColon Self "CALLABLE" := {
     Notation.double_colon := CALLABLE;
   }.
   
   Definition PAYABLE := Pure false.
   
-  Global Instance AssociatedFunction_PAYABLE `{H : State.Trait} :
+  Global Instance AssociatedFunction_PAYABLE :
     Notation.DoubleColon Self "PAYABLE" := {
     Notation.double_colon := PAYABLE;
   }.
   
   Definition SELECTOR := Pure [ 155; 174; 157; 94 ].
   
-  Global Instance AssociatedFunction_SELECTOR `{H : State.Trait} :
+  Global Instance AssociatedFunction_SELECTOR :
     Notation.DoubleColon Self "SELECTOR" := {
     Notation.double_colon := SELECTOR;
   }.
   
   Definition LABEL := Pure "new".
   
-  Global Instance AssociatedFunction_LABEL `{H : State.Trait} :
+  Global Instance AssociatedFunction_LABEL :
     Notation.DoubleColon Self "LABEL" := {
     Notation.double_colon := LABEL;
   }.
   
   Global Instance I :
       ink.reflect.dispatch.DispatchableConstructorInfo.Trait Self := {
-    ink.reflect.dispatch.DispatchableConstructorInfo.IS_RESULT
-      `{H : State.Trait}
-      :=
-      IS_RESULT;
-    ink.reflect.dispatch.DispatchableConstructorInfo.CALLABLE
-      `{H : State.Trait}
-      :=
-      CALLABLE;
-    ink.reflect.dispatch.DispatchableConstructorInfo.PAYABLE
-      `{H : State.Trait}
-      :=
-      PAYABLE;
-    ink.reflect.dispatch.DispatchableConstructorInfo.SELECTOR
-      `{H : State.Trait}
-      :=
-      SELECTOR;
-    ink.reflect.dispatch.DispatchableConstructorInfo.LABEL
-      `{H : State.Trait}
-      :=
-      LABEL;
+    ink.reflect.dispatch.DispatchableConstructorInfo.IS_RESULT := IS_RESULT;
+    ink.reflect.dispatch.DispatchableConstructorInfo.CALLABLE := CALLABLE;
+    ink.reflect.dispatch.DispatchableConstructorInfo.PAYABLE := PAYABLE;
+    ink.reflect.dispatch.DispatchableConstructorInfo.SELECTOR := SELECTOR;
+    ink.reflect.dispatch.DispatchableConstructorInfo.LABEL := LABEL;
   }.
 End Impl_ink_reflect_dispatch_DispatchableConstructorInfo_for_erc20_erc20_Erc20.
 
@@ -2342,61 +2102,46 @@ Module Impl_ink_reflect_dispatch_DispatchableMessageInfo_for_erc20_erc20_Erc20.
     CALLABLE := Pure
       (fun storage _ => erc20.erc20.Erc20::["total_supply"] storage).
   
-  Global Instance AssociatedFunction_CALLABLE `{H : State.Trait} :
+  Global Instance AssociatedFunction_CALLABLE :
     Notation.DoubleColon Self "CALLABLE" := {
     Notation.double_colon := CALLABLE;
   }.
   
   Definition SELECTOR := Pure [ 219; 99; 117; 168 ].
   
-  Global Instance AssociatedFunction_SELECTOR `{H : State.Trait} :
+  Global Instance AssociatedFunction_SELECTOR :
     Notation.DoubleColon Self "SELECTOR" := {
     Notation.double_colon := SELECTOR;
   }.
   
   Definition PAYABLE := Pure false.
   
-  Global Instance AssociatedFunction_PAYABLE `{H : State.Trait} :
+  Global Instance AssociatedFunction_PAYABLE :
     Notation.DoubleColon Self "PAYABLE" := {
     Notation.double_colon := PAYABLE;
   }.
   
   Definition MUTATES := Pure false.
   
-  Global Instance AssociatedFunction_MUTATES `{H : State.Trait} :
+  Global Instance AssociatedFunction_MUTATES :
     Notation.DoubleColon Self "MUTATES" := {
     Notation.double_colon := MUTATES;
   }.
   
   Definition LABEL := Pure "total_supply".
   
-  Global Instance AssociatedFunction_LABEL `{H : State.Trait} :
+  Global Instance AssociatedFunction_LABEL :
     Notation.DoubleColon Self "LABEL" := {
     Notation.double_colon := LABEL;
   }.
   
   Global Instance I :
       ink.reflect.dispatch.DispatchableMessageInfo.Trait Self := {
-    ink.reflect.dispatch.DispatchableMessageInfo.CALLABLE
-      `{H : State.Trait}
-      :=
-      CALLABLE;
-    ink.reflect.dispatch.DispatchableMessageInfo.MUTATES
-      `{H : State.Trait}
-      :=
-      MUTATES;
-    ink.reflect.dispatch.DispatchableMessageInfo.PAYABLE
-      `{H : State.Trait}
-      :=
-      PAYABLE;
-    ink.reflect.dispatch.DispatchableMessageInfo.SELECTOR
-      `{H : State.Trait}
-      :=
-      SELECTOR;
-    ink.reflect.dispatch.DispatchableMessageInfo.LABEL
-      `{H : State.Trait}
-      :=
-      LABEL;
+    ink.reflect.dispatch.DispatchableMessageInfo.CALLABLE := CALLABLE;
+    ink.reflect.dispatch.DispatchableMessageInfo.MUTATES := MUTATES;
+    ink.reflect.dispatch.DispatchableMessageInfo.PAYABLE := PAYABLE;
+    ink.reflect.dispatch.DispatchableMessageInfo.SELECTOR := SELECTOR;
+    ink.reflect.dispatch.DispatchableMessageInfo.LABEL := LABEL;
   }.
 End Impl_ink_reflect_dispatch_DispatchableMessageInfo_for_erc20_erc20_Erc20.
 
@@ -2414,61 +2159,46 @@ Module Impl_ink_reflect_dispatch_DispatchableMessageInfo_for_erc20_erc20_Erc20.
       (fun storage __ink_binding_0 =>
         erc20.erc20.Erc20::["balance_of"] storage __ink_binding_0).
   
-  Global Instance AssociatedFunction_CALLABLE `{H : State.Trait} :
+  Global Instance AssociatedFunction_CALLABLE :
     Notation.DoubleColon Self "CALLABLE" := {
     Notation.double_colon := CALLABLE;
   }.
   
   Definition SELECTOR := Pure [ 15; 117; 90; 86 ].
   
-  Global Instance AssociatedFunction_SELECTOR `{H : State.Trait} :
+  Global Instance AssociatedFunction_SELECTOR :
     Notation.DoubleColon Self "SELECTOR" := {
     Notation.double_colon := SELECTOR;
   }.
   
   Definition PAYABLE := Pure false.
   
-  Global Instance AssociatedFunction_PAYABLE `{H : State.Trait} :
+  Global Instance AssociatedFunction_PAYABLE :
     Notation.DoubleColon Self "PAYABLE" := {
     Notation.double_colon := PAYABLE;
   }.
   
   Definition MUTATES := Pure false.
   
-  Global Instance AssociatedFunction_MUTATES `{H : State.Trait} :
+  Global Instance AssociatedFunction_MUTATES :
     Notation.DoubleColon Self "MUTATES" := {
     Notation.double_colon := MUTATES;
   }.
   
   Definition LABEL := Pure "balance_of".
   
-  Global Instance AssociatedFunction_LABEL `{H : State.Trait} :
+  Global Instance AssociatedFunction_LABEL :
     Notation.DoubleColon Self "LABEL" := {
     Notation.double_colon := LABEL;
   }.
   
   Global Instance I :
       ink.reflect.dispatch.DispatchableMessageInfo.Trait Self := {
-    ink.reflect.dispatch.DispatchableMessageInfo.CALLABLE
-      `{H : State.Trait}
-      :=
-      CALLABLE;
-    ink.reflect.dispatch.DispatchableMessageInfo.MUTATES
-      `{H : State.Trait}
-      :=
-      MUTATES;
-    ink.reflect.dispatch.DispatchableMessageInfo.PAYABLE
-      `{H : State.Trait}
-      :=
-      PAYABLE;
-    ink.reflect.dispatch.DispatchableMessageInfo.SELECTOR
-      `{H : State.Trait}
-      :=
-      SELECTOR;
-    ink.reflect.dispatch.DispatchableMessageInfo.LABEL
-      `{H : State.Trait}
-      :=
-      LABEL;
+    ink.reflect.dispatch.DispatchableMessageInfo.CALLABLE := CALLABLE;
+    ink.reflect.dispatch.DispatchableMessageInfo.MUTATES := MUTATES;
+    ink.reflect.dispatch.DispatchableMessageInfo.PAYABLE := PAYABLE;
+    ink.reflect.dispatch.DispatchableMessageInfo.SELECTOR := SELECTOR;
+    ink.reflect.dispatch.DispatchableMessageInfo.LABEL := LABEL;
   }.
 End Impl_ink_reflect_dispatch_DispatchableMessageInfo_for_erc20_erc20_Erc20.
 
@@ -2489,61 +2219,46 @@ Module Impl_ink_reflect_dispatch_DispatchableMessageInfo_for_erc20_erc20_Erc20.
           __ink_binding_0
           __ink_binding_1).
   
-  Global Instance AssociatedFunction_CALLABLE `{H : State.Trait} :
+  Global Instance AssociatedFunction_CALLABLE :
     Notation.DoubleColon Self "CALLABLE" := {
     Notation.double_colon := CALLABLE;
   }.
   
   Definition SELECTOR := Pure [ 106; 0; 22; 94 ].
   
-  Global Instance AssociatedFunction_SELECTOR `{H : State.Trait} :
+  Global Instance AssociatedFunction_SELECTOR :
     Notation.DoubleColon Self "SELECTOR" := {
     Notation.double_colon := SELECTOR;
   }.
   
   Definition PAYABLE := Pure false.
   
-  Global Instance AssociatedFunction_PAYABLE `{H : State.Trait} :
+  Global Instance AssociatedFunction_PAYABLE :
     Notation.DoubleColon Self "PAYABLE" := {
     Notation.double_colon := PAYABLE;
   }.
   
   Definition MUTATES := Pure false.
   
-  Global Instance AssociatedFunction_MUTATES `{H : State.Trait} :
+  Global Instance AssociatedFunction_MUTATES :
     Notation.DoubleColon Self "MUTATES" := {
     Notation.double_colon := MUTATES;
   }.
   
   Definition LABEL := Pure "allowance".
   
-  Global Instance AssociatedFunction_LABEL `{H : State.Trait} :
+  Global Instance AssociatedFunction_LABEL :
     Notation.DoubleColon Self "LABEL" := {
     Notation.double_colon := LABEL;
   }.
   
   Global Instance I :
       ink.reflect.dispatch.DispatchableMessageInfo.Trait Self := {
-    ink.reflect.dispatch.DispatchableMessageInfo.CALLABLE
-      `{H : State.Trait}
-      :=
-      CALLABLE;
-    ink.reflect.dispatch.DispatchableMessageInfo.MUTATES
-      `{H : State.Trait}
-      :=
-      MUTATES;
-    ink.reflect.dispatch.DispatchableMessageInfo.PAYABLE
-      `{H : State.Trait}
-      :=
-      PAYABLE;
-    ink.reflect.dispatch.DispatchableMessageInfo.SELECTOR
-      `{H : State.Trait}
-      :=
-      SELECTOR;
-    ink.reflect.dispatch.DispatchableMessageInfo.LABEL
-      `{H : State.Trait}
-      :=
-      LABEL;
+    ink.reflect.dispatch.DispatchableMessageInfo.CALLABLE := CALLABLE;
+    ink.reflect.dispatch.DispatchableMessageInfo.MUTATES := MUTATES;
+    ink.reflect.dispatch.DispatchableMessageInfo.PAYABLE := PAYABLE;
+    ink.reflect.dispatch.DispatchableMessageInfo.SELECTOR := SELECTOR;
+    ink.reflect.dispatch.DispatchableMessageInfo.LABEL := LABEL;
   }.
 End Impl_ink_reflect_dispatch_DispatchableMessageInfo_for_erc20_erc20_Erc20.
 
@@ -2564,61 +2279,46 @@ Module Impl_ink_reflect_dispatch_DispatchableMessageInfo_for_erc20_erc20_Erc20.
           __ink_binding_0
           __ink_binding_1).
   
-  Global Instance AssociatedFunction_CALLABLE `{H : State.Trait} :
+  Global Instance AssociatedFunction_CALLABLE :
     Notation.DoubleColon Self "CALLABLE" := {
     Notation.double_colon := CALLABLE;
   }.
   
   Definition SELECTOR := Pure [ 132; 161; 93; 161 ].
   
-  Global Instance AssociatedFunction_SELECTOR `{H : State.Trait} :
+  Global Instance AssociatedFunction_SELECTOR :
     Notation.DoubleColon Self "SELECTOR" := {
     Notation.double_colon := SELECTOR;
   }.
   
   Definition PAYABLE := Pure false.
   
-  Global Instance AssociatedFunction_PAYABLE `{H : State.Trait} :
+  Global Instance AssociatedFunction_PAYABLE :
     Notation.DoubleColon Self "PAYABLE" := {
     Notation.double_colon := PAYABLE;
   }.
   
   Definition MUTATES := Pure true.
   
-  Global Instance AssociatedFunction_MUTATES `{H : State.Trait} :
+  Global Instance AssociatedFunction_MUTATES :
     Notation.DoubleColon Self "MUTATES" := {
     Notation.double_colon := MUTATES;
   }.
   
   Definition LABEL := Pure "transfer".
   
-  Global Instance AssociatedFunction_LABEL `{H : State.Trait} :
+  Global Instance AssociatedFunction_LABEL :
     Notation.DoubleColon Self "LABEL" := {
     Notation.double_colon := LABEL;
   }.
   
   Global Instance I :
       ink.reflect.dispatch.DispatchableMessageInfo.Trait Self := {
-    ink.reflect.dispatch.DispatchableMessageInfo.CALLABLE
-      `{H : State.Trait}
-      :=
-      CALLABLE;
-    ink.reflect.dispatch.DispatchableMessageInfo.MUTATES
-      `{H : State.Trait}
-      :=
-      MUTATES;
-    ink.reflect.dispatch.DispatchableMessageInfo.PAYABLE
-      `{H : State.Trait}
-      :=
-      PAYABLE;
-    ink.reflect.dispatch.DispatchableMessageInfo.SELECTOR
-      `{H : State.Trait}
-      :=
-      SELECTOR;
-    ink.reflect.dispatch.DispatchableMessageInfo.LABEL
-      `{H : State.Trait}
-      :=
-      LABEL;
+    ink.reflect.dispatch.DispatchableMessageInfo.CALLABLE := CALLABLE;
+    ink.reflect.dispatch.DispatchableMessageInfo.MUTATES := MUTATES;
+    ink.reflect.dispatch.DispatchableMessageInfo.PAYABLE := PAYABLE;
+    ink.reflect.dispatch.DispatchableMessageInfo.SELECTOR := SELECTOR;
+    ink.reflect.dispatch.DispatchableMessageInfo.LABEL := LABEL;
   }.
 End Impl_ink_reflect_dispatch_DispatchableMessageInfo_for_erc20_erc20_Erc20.
 
@@ -2636,61 +2336,46 @@ Module Impl_ink_reflect_dispatch_DispatchableMessageInfo_for_erc20_erc20_Erc20.
       (fun storage (__ink_binding_0, __ink_binding_1) =>
         erc20.erc20.Erc20::["approve"] storage __ink_binding_0 __ink_binding_1).
   
-  Global Instance AssociatedFunction_CALLABLE `{H : State.Trait} :
+  Global Instance AssociatedFunction_CALLABLE :
     Notation.DoubleColon Self "CALLABLE" := {
     Notation.double_colon := CALLABLE;
   }.
   
   Definition SELECTOR := Pure [ 104; 18; 102; 160 ].
   
-  Global Instance AssociatedFunction_SELECTOR `{H : State.Trait} :
+  Global Instance AssociatedFunction_SELECTOR :
     Notation.DoubleColon Self "SELECTOR" := {
     Notation.double_colon := SELECTOR;
   }.
   
   Definition PAYABLE := Pure false.
   
-  Global Instance AssociatedFunction_PAYABLE `{H : State.Trait} :
+  Global Instance AssociatedFunction_PAYABLE :
     Notation.DoubleColon Self "PAYABLE" := {
     Notation.double_colon := PAYABLE;
   }.
   
   Definition MUTATES := Pure true.
   
-  Global Instance AssociatedFunction_MUTATES `{H : State.Trait} :
+  Global Instance AssociatedFunction_MUTATES :
     Notation.DoubleColon Self "MUTATES" := {
     Notation.double_colon := MUTATES;
   }.
   
   Definition LABEL := Pure "approve".
   
-  Global Instance AssociatedFunction_LABEL `{H : State.Trait} :
+  Global Instance AssociatedFunction_LABEL :
     Notation.DoubleColon Self "LABEL" := {
     Notation.double_colon := LABEL;
   }.
   
   Global Instance I :
       ink.reflect.dispatch.DispatchableMessageInfo.Trait Self := {
-    ink.reflect.dispatch.DispatchableMessageInfo.CALLABLE
-      `{H : State.Trait}
-      :=
-      CALLABLE;
-    ink.reflect.dispatch.DispatchableMessageInfo.MUTATES
-      `{H : State.Trait}
-      :=
-      MUTATES;
-    ink.reflect.dispatch.DispatchableMessageInfo.PAYABLE
-      `{H : State.Trait}
-      :=
-      PAYABLE;
-    ink.reflect.dispatch.DispatchableMessageInfo.SELECTOR
-      `{H : State.Trait}
-      :=
-      SELECTOR;
-    ink.reflect.dispatch.DispatchableMessageInfo.LABEL
-      `{H : State.Trait}
-      :=
-      LABEL;
+    ink.reflect.dispatch.DispatchableMessageInfo.CALLABLE := CALLABLE;
+    ink.reflect.dispatch.DispatchableMessageInfo.MUTATES := MUTATES;
+    ink.reflect.dispatch.DispatchableMessageInfo.PAYABLE := PAYABLE;
+    ink.reflect.dispatch.DispatchableMessageInfo.SELECTOR := SELECTOR;
+    ink.reflect.dispatch.DispatchableMessageInfo.LABEL := LABEL;
   }.
 End Impl_ink_reflect_dispatch_DispatchableMessageInfo_for_erc20_erc20_Erc20.
 
@@ -2713,61 +2398,46 @@ Module Impl_ink_reflect_dispatch_DispatchableMessageInfo_for_erc20_erc20_Erc20.
           __ink_binding_1
           __ink_binding_2).
   
-  Global Instance AssociatedFunction_CALLABLE `{H : State.Trait} :
+  Global Instance AssociatedFunction_CALLABLE :
     Notation.DoubleColon Self "CALLABLE" := {
     Notation.double_colon := CALLABLE;
   }.
   
   Definition SELECTOR := Pure [ 11; 57; 111; 24 ].
   
-  Global Instance AssociatedFunction_SELECTOR `{H : State.Trait} :
+  Global Instance AssociatedFunction_SELECTOR :
     Notation.DoubleColon Self "SELECTOR" := {
     Notation.double_colon := SELECTOR;
   }.
   
   Definition PAYABLE := Pure false.
   
-  Global Instance AssociatedFunction_PAYABLE `{H : State.Trait} :
+  Global Instance AssociatedFunction_PAYABLE :
     Notation.DoubleColon Self "PAYABLE" := {
     Notation.double_colon := PAYABLE;
   }.
   
   Definition MUTATES := Pure true.
   
-  Global Instance AssociatedFunction_MUTATES `{H : State.Trait} :
+  Global Instance AssociatedFunction_MUTATES :
     Notation.DoubleColon Self "MUTATES" := {
     Notation.double_colon := MUTATES;
   }.
   
   Definition LABEL := Pure "transfer_from".
   
-  Global Instance AssociatedFunction_LABEL `{H : State.Trait} :
+  Global Instance AssociatedFunction_LABEL :
     Notation.DoubleColon Self "LABEL" := {
     Notation.double_colon := LABEL;
   }.
   
   Global Instance I :
       ink.reflect.dispatch.DispatchableMessageInfo.Trait Self := {
-    ink.reflect.dispatch.DispatchableMessageInfo.CALLABLE
-      `{H : State.Trait}
-      :=
-      CALLABLE;
-    ink.reflect.dispatch.DispatchableMessageInfo.MUTATES
-      `{H : State.Trait}
-      :=
-      MUTATES;
-    ink.reflect.dispatch.DispatchableMessageInfo.PAYABLE
-      `{H : State.Trait}
-      :=
-      PAYABLE;
-    ink.reflect.dispatch.DispatchableMessageInfo.SELECTOR
-      `{H : State.Trait}
-      :=
-      SELECTOR;
-    ink.reflect.dispatch.DispatchableMessageInfo.LABEL
-      `{H : State.Trait}
-      :=
-      LABEL;
+    ink.reflect.dispatch.DispatchableMessageInfo.CALLABLE := CALLABLE;
+    ink.reflect.dispatch.DispatchableMessageInfo.MUTATES := MUTATES;
+    ink.reflect.dispatch.DispatchableMessageInfo.PAYABLE := PAYABLE;
+    ink.reflect.dispatch.DispatchableMessageInfo.SELECTOR := SELECTOR;
+    ink.reflect.dispatch.DispatchableMessageInfo.LABEL := LABEL;
   }.
 End Impl_ink_reflect_dispatch_DispatchableMessageInfo_for_erc20_erc20_Erc20.
 
@@ -2782,11 +2452,8 @@ Module
   Definition Self := erc20.erc20._.__ink_ConstructorDecoder.
   
   Definition decode_dispatch
-      `{H : State.Trait}
       (input : mut_ref I)
-      :
-        M (H := H)
-          (core.result.Result Self ink.reflect.dispatch.DispatchError) :=
+      : M (core.result.Result Self ink.reflect.dispatch.DispatchError) :=
     let* α0 := parity_scale_codec.codec.Decode.decode input in
     let* α1 :=
       α0.["map_err"]
@@ -2822,21 +2489,18 @@ Module
           ink.reflect.dispatch.DispatchError.UnknownSelector)
     end.
   
-  Global Instance AssociatedFunction_decode_dispatch `{H : State.Trait} :
+  Global Instance AssociatedFunction_decode_dispatch :
     Notation.DoubleColon Self "decode_dispatch" := {
     Notation.double_colon := decode_dispatch;
   }.
   
   Global Instance I : ink.reflect.dispatch.DecodeDispatch.Trait Self := {
-    ink.reflect.dispatch.DecodeDispatch.decode_dispatch
-      `{H : State.Trait}
-      :=
-      decode_dispatch;
+    ink.reflect.dispatch.DecodeDispatch.decode_dispatch := decode_dispatch;
   }.
 End
   Impl_ink_reflect_dispatch_DecodeDispatch_for_erc20_erc20_____ink_ConstructorDecoder.
 
-Definition CONSTRUCTOR_0 `{H : State.Trait} : list Root.core.primitive.u8 :=
+Definition CONSTRUCTOR_0 : list Root.core.primitive.u8 :=
   run (Pure ink.reflect.dispatch.DispatchableConstructorInfo.SELECTOR).
 
 Module
@@ -2844,19 +2508,18 @@ Module
   Definition Self := erc20.erc20._.__ink_ConstructorDecoder.
   
   Definition decode
-      `{H : State.Trait}
       (input : mut_ref I)
-      : M (H := H) (core.result.Result Self parity_scale_codec.error.Error) :=
+      : M (core.result.Result Self parity_scale_codec.error.Error) :=
     let* α0 := ink.reflect.dispatch.DecodeDispatch.decode_dispatch input in
     α0.["map_err"] core.convert.Into.into.
   
-  Global Instance AssociatedFunction_decode `{H : State.Trait} :
+  Global Instance AssociatedFunction_decode :
     Notation.DoubleColon Self "decode" := {
     Notation.double_colon := decode;
   }.
   
   Global Instance I : parity_scale_codec.codec.Decode.Trait Self := {
-    parity_scale_codec.codec.Decode.decode `{H : State.Trait} := decode;
+    parity_scale_codec.codec.Decode.decode := decode;
   }.
 End
   Impl_parity_scale_codec_codec_Decode_for_erc20_erc20_____ink_ConstructorDecoder.
@@ -2866,11 +2529,8 @@ Module
   Definition Self := erc20.erc20._.__ink_ConstructorDecoder.
   
   Definition execute_dispatchable
-      `{H : State.Trait}
       (self : Self)
-      :
-        M (H := H)
-          (core.result.Result unit ink.reflect.dispatch.DispatchError) :=
+      : M (core.result.Result unit ink.reflect.dispatch.DispatchError) :=
     match self with
     | ImplSelf.Constructor0.Build_t input =>
       let* _ :=
@@ -2883,7 +2543,7 @@ Module
         let* α2 := α0.["andb"] α1 in
         if (α2 : bool) then
           let* _ :=
-            let* α0 := ink.codegen.dispatch.execution.deny_payment tt in
+            let* α0 := ink.codegen.dispatch.execution.deny_payment  in
             let* α1 := LangItem α0 in
             match α1 with
             | Break {| Break.0 := residual; |} =>
@@ -2921,14 +2581,13 @@ Module
       Pure tt
     end.
   
-  Global Instance Method_execute_dispatchable `{H : State.Trait} :
+  Global Instance Method_execute_dispatchable :
     Notation.Dot "execute_dispatchable" := {
     Notation.dot := execute_dispatchable;
   }.
   
   Global Instance I : ink.reflect.dispatch.ExecuteDispatchable.Trait Self := {
     ink.reflect.dispatch.ExecuteDispatchable.execute_dispatchable
-      `{H : State.Trait}
       :=
       execute_dispatchable;
   }.
@@ -2962,11 +2621,8 @@ Module
   Definition Self := erc20.erc20._.__ink_MessageDecoder.
   
   Definition decode_dispatch
-      `{H : State.Trait}
       (input : mut_ref I)
-      :
-        M (H := H)
-          (core.result.Result Self ink.reflect.dispatch.DispatchError) :=
+      : M (core.result.Result Self ink.reflect.dispatch.DispatchError) :=
     let* α0 := parity_scale_codec.codec.Decode.decode input in
     let* α1 :=
       α0.["map_err"]
@@ -3082,36 +2738,33 @@ Module
           ink.reflect.dispatch.DispatchError.UnknownSelector)
     end.
   
-  Global Instance AssociatedFunction_decode_dispatch `{H : State.Trait} :
+  Global Instance AssociatedFunction_decode_dispatch :
     Notation.DoubleColon Self "decode_dispatch" := {
     Notation.double_colon := decode_dispatch;
   }.
   
   Global Instance I : ink.reflect.dispatch.DecodeDispatch.Trait Self := {
-    ink.reflect.dispatch.DecodeDispatch.decode_dispatch
-      `{H : State.Trait}
-      :=
-      decode_dispatch;
+    ink.reflect.dispatch.DecodeDispatch.decode_dispatch := decode_dispatch;
   }.
 End
   Impl_ink_reflect_dispatch_DecodeDispatch_for_erc20_erc20_____ink_MessageDecoder.
 
-Definition MESSAGE_0 `{H : State.Trait} : list Root.core.primitive.u8 :=
+Definition MESSAGE_0 : list Root.core.primitive.u8 :=
   run (Pure ink.reflect.dispatch.DispatchableMessageInfo.SELECTOR).
 
-Definition MESSAGE_1 `{H : State.Trait} : list Root.core.primitive.u8 :=
+Definition MESSAGE_1 : list Root.core.primitive.u8 :=
   run (Pure ink.reflect.dispatch.DispatchableMessageInfo.SELECTOR).
 
-Definition MESSAGE_2 `{H : State.Trait} : list Root.core.primitive.u8 :=
+Definition MESSAGE_2 : list Root.core.primitive.u8 :=
   run (Pure ink.reflect.dispatch.DispatchableMessageInfo.SELECTOR).
 
-Definition MESSAGE_3 `{H : State.Trait} : list Root.core.primitive.u8 :=
+Definition MESSAGE_3 : list Root.core.primitive.u8 :=
   run (Pure ink.reflect.dispatch.DispatchableMessageInfo.SELECTOR).
 
-Definition MESSAGE_4 `{H : State.Trait} : list Root.core.primitive.u8 :=
+Definition MESSAGE_4 : list Root.core.primitive.u8 :=
   run (Pure ink.reflect.dispatch.DispatchableMessageInfo.SELECTOR).
 
-Definition MESSAGE_5 `{H : State.Trait} : list Root.core.primitive.u8 :=
+Definition MESSAGE_5 : list Root.core.primitive.u8 :=
   run (Pure ink.reflect.dispatch.DispatchableMessageInfo.SELECTOR).
 
 Module
@@ -3119,27 +2772,25 @@ Module
   Definition Self := erc20.erc20._.__ink_MessageDecoder.
   
   Definition decode
-      `{H : State.Trait}
       (input : mut_ref I)
-      : M (H := H) (core.result.Result Self parity_scale_codec.error.Error) :=
+      : M (core.result.Result Self parity_scale_codec.error.Error) :=
     let* α0 := ink.reflect.dispatch.DecodeDispatch.decode_dispatch input in
     α0.["map_err"] core.convert.Into.into.
   
-  Global Instance AssociatedFunction_decode `{H : State.Trait} :
+  Global Instance AssociatedFunction_decode :
     Notation.DoubleColon Self "decode" := {
     Notation.double_colon := decode;
   }.
   
   Global Instance I : parity_scale_codec.codec.Decode.Trait Self := {
-    parity_scale_codec.codec.Decode.decode `{H : State.Trait} := decode;
+    parity_scale_codec.codec.Decode.decode := decode;
   }.
 End Impl_parity_scale_codec_codec_Decode_for_erc20_erc20_____ink_MessageDecoder.
 
 Definition push_contract
-    `{H : State.Trait}
     (contract : core.mem.manually_drop.ManuallyDrop erc20.erc20.Erc20)
     (mutates : bool)
-    : M (H := H) unit :=
+    : M unit :=
   if (mutates : bool) then
     let* _ :=
       ink_env.api.set_contract_storage
@@ -3154,11 +2805,8 @@ Module
   Definition Self := erc20.erc20._.__ink_MessageDecoder.
   
   Definition execute_dispatchable
-      `{H : State.Trait}
       (self : Self)
-      :
-        M (H := H)
-          (core.result.Result unit ink.reflect.dispatch.DispatchError) :=
+      : M (core.result.Result unit ink.reflect.dispatch.DispatchError) :=
     let key := ink_storage_traits.storage.StorageKey.KEY in
     let* contract :=
       let* α0 := ink_env.api.get_contract_storage (addr_of key) in
@@ -3210,7 +2858,7 @@ Module
           let* α2 := α0.["andb"] α1 in
           if (α2 : bool) then
             let* _ :=
-              let* α0 := ink.codegen.dispatch.execution.deny_payment tt in
+              let* α0 := ink.codegen.dispatch.execution.deny_payment  in
               let* α1 := LangItem α0 in
               match α1 with
               | Break {| Break.0 := residual; |} =>
@@ -3276,7 +2924,7 @@ Module
           let* α2 := α0.["andb"] α1 in
           if (α2 : bool) then
             let* _ :=
-              let* α0 := ink.codegen.dispatch.execution.deny_payment tt in
+              let* α0 := ink.codegen.dispatch.execution.deny_payment  in
               let* α1 := LangItem α0 in
               match α1 with
               | Break {| Break.0 := residual; |} =>
@@ -3342,7 +2990,7 @@ Module
           let* α2 := α0.["andb"] α1 in
           if (α2 : bool) then
             let* _ :=
-              let* α0 := ink.codegen.dispatch.execution.deny_payment tt in
+              let* α0 := ink.codegen.dispatch.execution.deny_payment  in
               let* α1 := LangItem α0 in
               match α1 with
               | Break {| Break.0 := residual; |} =>
@@ -3408,7 +3056,7 @@ Module
           let* α2 := α0.["andb"] α1 in
           if (α2 : bool) then
             let* _ :=
-              let* α0 := ink.codegen.dispatch.execution.deny_payment tt in
+              let* α0 := ink.codegen.dispatch.execution.deny_payment  in
               let* α1 := LangItem α0 in
               match α1 with
               | Break {| Break.0 := residual; |} =>
@@ -3474,7 +3122,7 @@ Module
           let* α2 := α0.["andb"] α1 in
           if (α2 : bool) then
             let* _ :=
-              let* α0 := ink.codegen.dispatch.execution.deny_payment tt in
+              let* α0 := ink.codegen.dispatch.execution.deny_payment  in
               let* α1 := LangItem α0 in
               match α1 with
               | Break {| Break.0 := residual; |} =>
@@ -3540,7 +3188,7 @@ Module
           let* α2 := α0.["andb"] α1 in
           if (α2 : bool) then
             let* _ :=
-              let* α0 := ink.codegen.dispatch.execution.deny_payment tt in
+              let* α0 := ink.codegen.dispatch.execution.deny_payment  in
               let* α1 := LangItem α0 in
               match α1 with
               | Break {| Break.0 := residual; |} =>
@@ -3578,14 +3226,13 @@ Module
       end in
     Pure tt.
   
-  Global Instance Method_execute_dispatchable `{H : State.Trait} :
+  Global Instance Method_execute_dispatchable :
     Notation.Dot "execute_dispatchable" := {
     Notation.dot := execute_dispatchable;
   }.
   
   Global Instance I : ink.reflect.dispatch.ExecuteDispatchable.Trait Self := {
     ink.reflect.dispatch.ExecuteDispatchable.execute_dispatchable
-      `{H : State.Trait}
       :=
       execute_dispatchable;
   }.
@@ -3602,33 +3249,27 @@ Module Impl_ink_reflect_dispatch_ContractMessageDecoder_for_erc20_erc20_Erc20.
   }.
 End Impl_ink_reflect_dispatch_ContractMessageDecoder_for_erc20_erc20_Erc20.
 
-Definition
-    _
-    `{H : State.Trait} :
-    ink.codegen.utils.same_type.IsSameType erc20.erc20.Erc20 :=
-  run ((ink.codegen.utils.same_type.IsSameType erc20.erc20.Erc20)::["new"] tt).
+Definition _ : ink.codegen.utils.same_type.IsSameType erc20.erc20.Erc20 :=
+  run ((ink.codegen.utils.same_type.IsSameType erc20.erc20.Erc20)::["new"] ).
 
 Module Impl_erc20_erc20_Erc20.
   Definition Self := erc20.erc20.Erc20.
   
-  Definition new
-      `{H : State.Trait}
-      (total_supply : erc20.erc20.Balance)
-      : M (H := H) Self :=
-    let* balances := ink_storage.lazy.mapping.Mapping::["default"] tt in
+  Definition new (total_supply : erc20.erc20.Balance) : M Self :=
+    let* balances := ink_storage.lazy.mapping.Mapping::["default"]  in
     let* caller :=
-      let* α0 := Self::["env"] tt in
+      let* α0 := Self::["env"]  in
       α0.["caller"] in
     let* _ := balances.["insert"] caller (addr_of total_supply) in
     let* _ :=
-      let* α0 := Self::["env"] tt in
+      let* α0 := Self::["env"]  in
       α0.["emit_event"]
         {|
           erc20.erc20.Transfer.from := core.option.Option.None;
           erc20.erc20.Transfer.to := core.option.Option.Some caller;
           erc20.erc20.Transfer.value := total_supply;
         |} in
-    let* α0 := core.default.Default.default tt in
+    let* α0 := core.default.Default.default  in
     Pure
       {|
         Self.total_supply := total_supply;
@@ -3636,69 +3277,57 @@ Module Impl_erc20_erc20_Erc20.
         Self.allowances := α0;
       |}.
   
-  Global Instance AssociatedFunction_new `{H : State.Trait} :
-    Notation.DoubleColon Self "new" := {
+  Global Instance AssociatedFunction_new : Notation.DoubleColon Self "new" := {
     Notation.double_colon := new;
   }.
   
-  Definition total_supply
-      `{H : State.Trait}
-      (self : ref Self)
-      : M (H := H) erc20.erc20.Balance :=
+  Definition total_supply (self : ref Self) : M erc20.erc20.Balance :=
     Pure self.["total_supply"].
   
-  Global Instance Method_total_supply `{H : State.Trait} :
-    Notation.Dot "total_supply" := {
+  Global Instance Method_total_supply : Notation.Dot "total_supply" := {
     Notation.dot := total_supply;
   }.
   
   Definition balance_of
-      `{H : State.Trait}
       (self : ref Self)
       (owner : erc20.erc20.AccountId)
-      : M (H := H) erc20.erc20.Balance :=
+      : M erc20.erc20.Balance :=
     self.["balance_of_impl"] (addr_of owner).
   
-  Global Instance Method_balance_of `{H : State.Trait} :
-    Notation.Dot "balance_of" := {
+  Global Instance Method_balance_of : Notation.Dot "balance_of" := {
     Notation.dot := balance_of;
   }.
   
   Definition allowance
-      `{H : State.Trait}
       (self : ref Self)
       (owner : erc20.erc20.AccountId)
       (spender : erc20.erc20.AccountId)
-      : M (H := H) erc20.erc20.Balance :=
+      : M erc20.erc20.Balance :=
     self.["allowance_impl"] (addr_of owner) (addr_of spender).
   
-  Global Instance Method_allowance `{H : State.Trait} :
-    Notation.Dot "allowance" := {
+  Global Instance Method_allowance : Notation.Dot "allowance" := {
     Notation.dot := allowance;
   }.
   
   Definition transfer
-      `{H : State.Trait}
       (self : mut_ref Self)
       (to : erc20.erc20.AccountId)
       (value : erc20.erc20.Balance)
-      : M (H := H) (erc20.erc20.Result unit) :=
+      : M (erc20.erc20.Result unit) :=
     let* from :=
       let* α0 := self.["env"] in
       α0.["caller"] in
     self.["transfer_from_to"] (addr_of from) (addr_of to) value.
   
-  Global Instance Method_transfer `{H : State.Trait} :
-    Notation.Dot "transfer" := {
+  Global Instance Method_transfer : Notation.Dot "transfer" := {
     Notation.dot := transfer;
   }.
   
   Definition approve
-      `{H : State.Trait}
       (self : mut_ref Self)
       (spender : erc20.erc20.AccountId)
       (value : erc20.erc20.Balance)
-      : M (H := H) (erc20.erc20.Result unit) :=
+      : M (erc20.erc20.Result unit) :=
     let* owner :=
       let* α0 := self.["env"] in
       α0.["caller"] in
@@ -3716,18 +3345,16 @@ Module Impl_erc20_erc20_Erc20.
         |} in
     Pure (core.result.Result.Ok tt).
   
-  Global Instance Method_approve `{H : State.Trait} :
-    Notation.Dot "approve" := {
+  Global Instance Method_approve : Notation.Dot "approve" := {
     Notation.dot := approve;
   }.
   
   Definition transfer_from
-      `{H : State.Trait}
       (self : mut_ref Self)
       (from : erc20.erc20.AccountId)
       (to : erc20.erc20.AccountId)
       (value : erc20.erc20.Balance)
-      : M (H := H) (erc20.erc20.Result unit) :=
+      : M (erc20.erc20.Result unit) :=
     let* caller :=
       let* α0 := self.["env"] in
       α0.["caller"] in
@@ -3754,45 +3381,39 @@ Module Impl_erc20_erc20_Erc20.
         (addr_of α0) in
     Pure (core.result.Result.Ok tt).
   
-  Global Instance Method_transfer_from `{H : State.Trait} :
-    Notation.Dot "transfer_from" := {
+  Global Instance Method_transfer_from : Notation.Dot "transfer_from" := {
     Notation.dot := transfer_from;
   }.
   
   Definition balance_of_impl
-      `{H : State.Trait}
       (self : ref Self)
       (owner : ref erc20.erc20.AccountId)
-      : M (H := H) erc20.erc20.Balance :=
+      : M erc20.erc20.Balance :=
     let* α0 := self.["balances"].["get"] owner in
     α0.["unwrap_or_default"].
   
-  Global Instance Method_balance_of_impl `{H : State.Trait} :
-    Notation.Dot "balance_of_impl" := {
+  Global Instance Method_balance_of_impl : Notation.Dot "balance_of_impl" := {
     Notation.dot := balance_of_impl;
   }.
   
   Definition allowance_impl
-      `{H : State.Trait}
       (self : ref Self)
       (owner : ref erc20.erc20.AccountId)
       (spender : ref erc20.erc20.AccountId)
-      : M (H := H) erc20.erc20.Balance :=
+      : M erc20.erc20.Balance :=
     let* α0 := self.["allowances"].["get"] (owner, spender) in
     α0.["unwrap_or_default"].
   
-  Global Instance Method_allowance_impl `{H : State.Trait} :
-    Notation.Dot "allowance_impl" := {
+  Global Instance Method_allowance_impl : Notation.Dot "allowance_impl" := {
     Notation.dot := allowance_impl;
   }.
   
   Definition transfer_from_to
-      `{H : State.Trait}
       (self : mut_ref Self)
       (from : ref erc20.erc20.AccountId)
       (to : ref erc20.erc20.AccountId)
       (value : erc20.erc20.Balance)
-      : M (H := H) (erc20.erc20.Result unit) :=
+      : M (erc20.erc20.Result unit) :=
     let* from_balance := self.["balance_of_impl"] from in
     let* _ :=
       let* α0 := from_balance.["lt"] value in
@@ -3819,8 +3440,7 @@ Module Impl_erc20_erc20_Erc20.
         |} in
     Pure (core.result.Result.Ok tt).
   
-  Global Instance Method_transfer_from_to `{H : State.Trait} :
-    Notation.Dot "transfer_from_to" := {
+  Global Instance Method_transfer_from_to : Notation.Dot "transfer_from_to" := {
     Notation.dot := transfer_from_to;
   }.
 End Impl_erc20_erc20_Erc20.
@@ -3839,31 +3459,22 @@ Definition CallBuilder : Set := CallBuilder.t.
 Module Impl_core_fmt_Debug_for_erc20_erc20___CallBuilder.
   Definition Self := erc20.erc20._.CallBuilder.
   
-  Parameter debug_struct_field1_finish : core.fmt.Formatter -> string -> 
-    string -> erc20_erc20_AccountId -> 
-    M (H := H) core.fmt.Result.
-  
-  Global Instance Deb_debug_struct_field1_finish : Notation.DoubleColon
-    core.fmt.Formatter "debug_struct_field1_finish" := {
-    Notation.double_colon := debug_struct_field1_finish; }.
-  
   Definition fmt
-      `{H : State.Trait}
       (self : ref Self)
       (f : mut_ref core.fmt.Formatter)
-      : M (H := H) core.fmt.Result :=
+      : M core.fmt.Result :=
     core.fmt.Formatter::["debug_struct_field1_finish"]
       f
       "CallBuilder"
       "account_id"
       (addr_of (addr_of self.["account_id"])).
   
-  Global Instance Method_fmt `{H : State.Trait} : Notation.Dot "fmt" := {
+  Global Instance Method_fmt : Notation.Dot "fmt" := {
     Notation.dot := fmt;
   }.
   
   Global Instance I : core.fmt.Debug.Trait Self := {
-    core.fmt.Debug.fmt `{H : State.Trait} := fmt;
+    core.fmt.Debug.fmt := fmt;
   }.
 End Impl_core_fmt_Debug_for_erc20_erc20___CallBuilder.
 
@@ -3871,41 +3482,33 @@ Module Impl_parity_scale_codec_codec_Encode_for_erc20_erc20___CallBuilder.
   Definition Self := erc20.erc20._.CallBuilder.
   
   Definition encode_to
-      `{H : State.Trait}
       (self : ref Self)
       (__codec_dest_edqy : mut_ref __CodecOutputEdqy)
-      : M (H := H) unit :=
+      : M unit :=
     parity_scale_codec.codec.Encode.encode_to
       (addr_of (addr_of self.["account_id"]))
       __codec_dest_edqy.
   
-  Global Instance Method_encode_to `{H : State.Trait} :
-    Notation.Dot "encode_to" := {
+  Global Instance Method_encode_to : Notation.Dot "encode_to" := {
     Notation.dot := encode_to;
   }.
   
   Definition encode
-      `{H : State.Trait}
       (self : ref Self)
-      : M (H := H) (alloc.vec.Vec Root.core.primitive.u8) :=
+      : M (alloc.vec.Vec Root.core.primitive.u8) :=
     parity_scale_codec.codec.Encode.encode
       (addr_of (addr_of self.["account_id"])).
   
-  Global Instance Method_encode `{H : State.Trait} : Notation.Dot "encode" := {
+  Global Instance Method_encode : Notation.Dot "encode" := {
     Notation.dot := encode;
   }.
   
-  Definition using_encoded
-      `{H : State.Trait}
-      (self : ref Self)
-      (f : F)
-      : M (H := H) R :=
+  Definition using_encoded (self : ref Self) (f : F) : M R :=
     parity_scale_codec.codec.Encode.using_encoded
       (addr_of (addr_of self.["account_id"]))
       f.
   
-  Global Instance Method_using_encoded `{H : State.Trait} :
-    Notation.Dot "using_encoded" := {
+  Global Instance Method_using_encoded : Notation.Dot "using_encoded" := {
     Notation.dot := using_encoded;
   }.
   
@@ -3926,9 +3529,8 @@ Module Impl_parity_scale_codec_codec_Decode_for_erc20_erc20___CallBuilder.
   Definition Self := erc20.erc20._.CallBuilder.
   
   Definition decode
-      `{H : State.Trait}
       (__codec_input_edqy : mut_ref __CodecInputEdqy)
-      : M (H := H) (core.result.Result Self parity_scale_codec.error.Error) :=
+      : M (core.result.Result Self parity_scale_codec.error.Error) :=
     let* __codec_res_edqy :=
       parity_scale_codec.codec.Decode.decode __codec_input_edqy in
     let* α0 :=
@@ -3941,23 +3543,22 @@ Module Impl_parity_scale_codec_codec_Decode_for_erc20_erc20___CallBuilder.
     Pure
       (core.result.Result.Ok {| erc20.erc20._.CallBuilder.account_id := α0; |}).
   
-  Global Instance AssociatedFunction_decode `{H : State.Trait} :
+  Global Instance AssociatedFunction_decode :
     Notation.DoubleColon Self "decode" := {
     Notation.double_colon := decode;
   }.
   
   Definition decode_into
-      `{H : State.Trait}
       (__codec_input_edqy : mut_ref __CodecInputEdqy)
       (dst_ : mut_ref (core.mem.maybe_uninit.MaybeUninit Self))
       :
-        M (H := H)
+        M
           (core.result.Result
             parity_scale_codec.decode_finished.DecodeFinished
             parity_scale_codec.error.Error) :=
     let* _ :=
-      let* α0 := core.mem.size_of tt in
-      let* α1 := core.mem.size_of tt in
+      let* α0 := core.mem.size_of  in
+      let* α1 := core.mem.size_of  in
       match (addr_of α0, addr_of α1) with
       | (left_val, right_val) =>
         let* α0 := left_val.["deref"] in
@@ -3979,7 +3580,7 @@ Module Impl_parity_scale_codec_codec_Decode_for_erc20_erc20___CallBuilder.
           Pure tt
       end in
     let* _ :=
-      let* α0 := core.mem.size_of tt in
+      let* α0 := core.mem.size_of  in
       let* α1 := α0.["gt"] 0 in
       let* α2 :=
         if (α1 : bool) then
@@ -4013,35 +3614,31 @@ Module Impl_parity_scale_codec_codec_Decode_for_erc20_erc20___CallBuilder.
       Pure tt in
     let* α0 :=
       parity_scale_codec.decode_finished.DecodeFinished::["assert_decoding_finished"]
-        tt in
+         in
     Pure (core.result.Result.Ok α0).
   
-  Global Instance AssociatedFunction_decode_into `{H : State.Trait} :
+  Global Instance AssociatedFunction_decode_into :
     Notation.DoubleColon Self "decode_into" := {
     Notation.double_colon := decode_into;
   }.
   
   Global Instance I : parity_scale_codec.codec.Decode.Trait Self := {
-    parity_scale_codec.codec.Decode.decode `{H : State.Trait} := decode;
+    parity_scale_codec.codec.Decode.decode := decode;
   }.
 End Impl_parity_scale_codec_codec_Decode_for_erc20_erc20___CallBuilder.
 
 Module Impl_core_hash_Hash_for_erc20_erc20___CallBuilder.
   Definition Self := erc20.erc20._.CallBuilder.
   
-  Definition hash
-      `{H : State.Trait}
-      (self : ref Self)
-      (state : mut_ref __H)
-      : M (H := H) unit :=
+  Definition hash (self : ref Self) (state : mut_ref __H) : M unit :=
     core.hash.Hash.hash (addr_of self.["account_id"]) state.
   
-  Global Instance Method_hash `{H : State.Trait} : Notation.Dot "hash" := {
+  Global Instance Method_hash : Notation.Dot "hash" := {
     Notation.dot := hash;
   }.
   
   Global Instance I : core.hash.Hash.Trait Self := {
-    core.hash.Hash.hash `{H : State.Trait} := hash;
+    core.hash.Hash.hash := hash;
   }.
 End Impl_core_hash_Hash_for_erc20_erc20___CallBuilder.
 
@@ -4056,18 +3653,17 @@ Module Impl_core_cmp_PartialEq_for_erc20_erc20___CallBuilder.
   Definition Self := erc20.erc20._.CallBuilder.
   
   Definition eq
-      `{H : State.Trait}
       (self : ref Self)
       (other : ref erc20.erc20._.CallBuilder)
-      : M (H := H) bool :=
+      : M bool :=
     self.["account_id"].["eq"] other.["account_id"].
   
-  Global Instance Method_eq `{H : State.Trait} : Notation.Dot "eq" := {
+  Global Instance Method_eq : Notation.Dot "eq" := {
     Notation.dot := eq;
   }.
   
   Global Instance I : core.cmp.PartialEq.Trait Self := {
-    core.cmp.PartialEq.eq `{H : State.Trait} := eq;
+    core.cmp.PartialEq.eq := eq;
   }.
 End Impl_core_cmp_PartialEq_for_erc20_erc20___CallBuilder.
 
@@ -4081,14 +3677,11 @@ End Impl_core_marker_StructuralEq_for_erc20_erc20___CallBuilder.
 Module Impl_core_cmp_Eq_for_erc20_erc20___CallBuilder.
   Definition Self := erc20.erc20._.CallBuilder.
   
-  Definition assert_receiver_is_total_eq
-      `{H : State.Trait}
-      (self : ref Self)
-      : M (H := H) unit :=
+  Definition assert_receiver_is_total_eq (self : ref Self) : M unit :=
     let _ := tt in
     Pure tt.
   
-  Global Instance Method_assert_receiver_is_total_eq `{H : State.Trait} :
+  Global Instance Method_assert_receiver_is_total_eq :
     Notation.Dot "assert_receiver_is_total_eq" := {
     Notation.dot := assert_receiver_is_total_eq;
   }.
@@ -4100,19 +3693,16 @@ End Impl_core_cmp_Eq_for_erc20_erc20___CallBuilder.
 Module Impl_core_clone_Clone_for_erc20_erc20___CallBuilder.
   Definition Self := erc20.erc20._.CallBuilder.
   
-  Definition clone
-      `{H : State.Trait}
-      (self : ref Self)
-      : M (H := H) erc20.erc20._.CallBuilder :=
+  Definition clone (self : ref Self) : M erc20.erc20._.CallBuilder :=
     let* α0 := core.clone.Clone.clone (addr_of self.["account_id"]) in
     Pure {| erc20.erc20._.CallBuilder.account_id := α0; |}.
   
-  Global Instance Method_clone `{H : State.Trait} : Notation.Dot "clone" := {
+  Global Instance Method_clone : Notation.Dot "clone" := {
     Notation.dot := clone;
   }.
   
   Global Instance I : core.clone.Clone.Trait Self := {
-    core.clone.Clone.clone `{H : State.Trait} := clone;
+    core.clone.Clone.clone := clone;
   }.
 End Impl_core_clone_Clone_for_erc20_erc20___CallBuilder.
 
@@ -4121,14 +3711,11 @@ Module Impl_scale_info_TypeInfo_for_erc20_erc20___CallBuilder.
   
   Definition Identity : Set := Self.
   
-  Definition type_info
-      `{H : State.Trait}
-      (_ : unit)
-      : M (H := H) scale_info.ty.Type :=
-    let* α0 := scale_info.ty.Type::["builder"] tt in
+  Definition type_info  : M scale_info.ty.Type :=
+    let* α0 := scale_info.ty.Type::["builder"]  in
     let* α1 := scale_info.ty.path.Path::["new"] "CallBuilder" "erc20::erc20" in
     let* α2 := α0.["path"] α1 in
-    let* α3 := alloc.vec.Vec::["new"] tt in
+    let* α3 := alloc.vec.Vec::["new"]  in
     let* α4 := α2.["type_params"] α3 in
     let* α5 :=
       α4.["docs"]
@@ -4139,7 +3726,7 @@ Module Impl_scale_info_TypeInfo_for_erc20_erc20___CallBuilder.
             "Implements the underlying on-chain calling of the ink! smart contract";
             "messages and trait implementations in a type safe way."
           ]) in
-    let* α6 := scale_info.build.Fields::["named"] tt in
+    let* α6 := scale_info.build.Fields::["named"]  in
     let* α7 :=
       α6.["field"]
         (fun f =>
@@ -4148,13 +3735,13 @@ Module Impl_scale_info_TypeInfo_for_erc20_erc20___CallBuilder.
           α1.["type_name"] "AccountId") in
     α5.["composite"] α7.
   
-  Global Instance AssociatedFunction_type_info `{H : State.Trait} :
+  Global Instance AssociatedFunction_type_info :
     Notation.DoubleColon Self "type_info" := {
     Notation.double_colon := type_info;
   }.
   
   Global Instance I : scale_info.TypeInfo.Trait Self := {
-    scale_info.TypeInfo.type_info `{H : State.Trait} := type_info;
+    scale_info.TypeInfo.type_info := type_info;
   }.
 End Impl_scale_info_TypeInfo_for_erc20_erc20___CallBuilder.
 
@@ -4163,21 +3750,20 @@ Module
   Definition Self := erc20.erc20._.CallBuilder.
   
   Definition layout
-      `{H : State.Trait}
       (__key : ref ink_primitives.key.Key)
-      : M (H := H) ink_metadata.layout.Layout :=
+      : M ink_metadata.layout.Layout :=
     let* α0 := ink_storage_traits.layout.StorageLayout.layout __key in
     let* α1 := ink_metadata.layout.FieldLayout::["new"] "account_id" α0 in
     let* α2 := ink_metadata.layout.StructLayout::["new"] "CallBuilder" [ α1 ] in
     Pure (ink_metadata.layout.Layout.Struct α2).
   
-  Global Instance AssociatedFunction_layout `{H : State.Trait} :
+  Global Instance AssociatedFunction_layout :
     Notation.DoubleColon Self "layout" := {
     Notation.double_colon := layout;
   }.
   
   Global Instance I : ink_storage_traits.layout.StorageLayout.Trait Self := {
-    ink_storage_traits.layout.StorageLayout.layout `{H : State.Trait} := layout;
+    ink_storage_traits.layout.StorageLayout.layout := layout;
   }.
 End Impl_ink_storage_traits_layout_StorageLayout_for_erc20_erc20___CallBuilder.
 
@@ -4204,13 +3790,10 @@ Module
   Impl_ink_env_call_create_builder_FromAccountId_for_erc20_erc20___CallBuilder.
   Definition Self := erc20.erc20._.CallBuilder.
   
-  Definition from_account_id
-      `{H : State.Trait}
-      (account_id : erc20.erc20.AccountId)
-      : M (H := H) Self :=
+  Definition from_account_id (account_id : erc20.erc20.AccountId) : M Self :=
     Pure {| Self.account_id := account_id; |}.
   
-  Global Instance AssociatedFunction_from_account_id `{H : State.Trait} :
+  Global Instance AssociatedFunction_from_account_id :
     Notation.DoubleColon Self "from_account_id" := {
     Notation.double_colon := from_account_id;
   }.
@@ -4220,7 +3803,6 @@ Module
         Self
         (T := erc20.erc20.Environment) := {
     ink_env.call.create_builder.FromAccountId.from_account_id
-      `{H : State.Trait}
       :=
       from_account_id;
   }.
@@ -4230,14 +3812,10 @@ End
 Module Impl_ink_contract_ref_ToAccountId_for_erc20_erc20___CallBuilder.
   Definition Self := erc20.erc20._.CallBuilder.
   
-  Definition to_account_id
-      `{H : State.Trait}
-      (self : ref Self)
-      : M (H := H) erc20.erc20.AccountId :=
+  Definition to_account_id (self : ref Self) : M erc20.erc20.AccountId :=
     core.clone.Clone.clone (addr_of self.["account_id"]).
   
-  Global Instance Method_to_account_id `{H : State.Trait} :
-    Notation.Dot "to_account_id" := {
+  Global Instance Method_to_account_id : Notation.Dot "to_account_id" := {
     Notation.dot := to_account_id;
   }.
   
@@ -4245,48 +3823,39 @@ Module Impl_ink_contract_ref_ToAccountId_for_erc20_erc20___CallBuilder.
       ink.contract_ref.ToAccountId.Trait
         Self
         (T := erc20.erc20.Environment) := {
-    ink.contract_ref.ToAccountId.to_account_id
-      `{H : State.Trait}
-      :=
-      to_account_id;
+    ink.contract_ref.ToAccountId.to_account_id := to_account_id;
   }.
 End Impl_ink_contract_ref_ToAccountId_for_erc20_erc20___CallBuilder.
 
 Module Impl_core_convert_AsRef_for_erc20_erc20___CallBuilder.
   Definition Self := erc20.erc20._.CallBuilder.
   
-  Definition as_ref
-      `{H : State.Trait}
-      (self : ref Self)
-      : M (H := H) (ref erc20.erc20.AccountId) :=
+  Definition as_ref (self : ref Self) : M (ref erc20.erc20.AccountId) :=
     Pure (addr_of self.["account_id"]).
   
-  Global Instance Method_as_ref `{H : State.Trait} : Notation.Dot "as_ref" := {
+  Global Instance Method_as_ref : Notation.Dot "as_ref" := {
     Notation.dot := as_ref;
   }.
   
   Global Instance I :
       core.convert.AsRef.Trait Self (T := erc20.erc20.AccountId) := {
-    core.convert.AsRef.as_ref `{H : State.Trait} := as_ref;
+    core.convert.AsRef.as_ref := as_ref;
   }.
 End Impl_core_convert_AsRef_for_erc20_erc20___CallBuilder.
 
 Module Impl_core_convert_AsMut_for_erc20_erc20___CallBuilder.
   Definition Self := erc20.erc20._.CallBuilder.
   
-  Definition as_mut
-      `{H : State.Trait}
-      (self : mut_ref Self)
-      : M (H := H) (mut_ref erc20.erc20.AccountId) :=
+  Definition as_mut (self : mut_ref Self) : M (mut_ref erc20.erc20.AccountId) :=
     Pure (addr_of self.["account_id"]).
   
-  Global Instance Method_as_mut `{H : State.Trait} : Notation.Dot "as_mut" := {
+  Global Instance Method_as_mut : Notation.Dot "as_mut" := {
     Notation.dot := as_mut;
   }.
   
   Global Instance I :
       core.convert.AsMut.Trait Self (T := erc20.erc20.AccountId) := {
-    core.convert.AsMut.as_mut `{H : State.Trait} := as_mut;
+    core.convert.AsMut.as_mut := as_mut;
   }.
 End Impl_core_convert_AsMut_for_erc20_erc20___CallBuilder.
 
@@ -4294,10 +3863,9 @@ Module Impl_erc20_erc20___CallBuilder.
   Definition Self := erc20.erc20._.CallBuilder.
   
   Definition total_supply
-      `{H : State.Trait}
       (self : ref Self)
       :
-        M (H := H)
+        M
           (ink_env.call.call_builder.CallBuilder
             erc20.erc20.Environment
             (ink_env.call.common.Set
@@ -4307,7 +3875,7 @@ Module Impl_erc20_erc20___CallBuilder.
                 ink_env.call.execution_input.EmptyArgumentList))
             (ink_env.call.common.Set
               (ink_env.call.common.ReturnType erc20.erc20.Balance))) :=
-    let* α0 := ink_env.call.call_builder.build_call tt in
+    let* α0 := ink_env.call.call_builder.build_call  in
     let* α1 := ink.contract_ref.ToAccountId.to_account_id self in
     let* α2 := α0.["call"] α1 in
     let* α3 := ink_env.call.selector.Selector::["new"] [ 219; 99; 117; 168 ] in
@@ -4315,17 +3883,15 @@ Module Impl_erc20_erc20___CallBuilder.
     let* α5 := α2.["exec_input"] α4 in
     α5.["returns"].
   
-  Global Instance Method_total_supply `{H : State.Trait} :
-    Notation.Dot "total_supply" := {
+  Global Instance Method_total_supply : Notation.Dot "total_supply" := {
     Notation.dot := total_supply;
   }.
   
   Definition balance_of
-      `{H : State.Trait}
       (self : ref Self)
       (__ink_binding_0 : erc20.erc20.AccountId)
       :
-        M (H := H)
+        M
           (ink_env.call.call_builder.CallBuilder
             erc20.erc20.Environment
             (ink_env.call.common.Set
@@ -4337,7 +3903,7 @@ Module Impl_erc20_erc20___CallBuilder.
                   ink_env.call.execution_input.EmptyArgumentList)))
             (ink_env.call.common.Set
               (ink_env.call.common.ReturnType erc20.erc20.Balance))) :=
-    let* α0 := ink_env.call.call_builder.build_call tt in
+    let* α0 := ink_env.call.call_builder.build_call  in
     let* α1 := ink.contract_ref.ToAccountId.to_account_id self in
     let* α2 := α0.["call"] α1 in
     let* α3 := ink_env.call.selector.Selector::["new"] [ 15; 117; 90; 86 ] in
@@ -4346,18 +3912,16 @@ Module Impl_erc20_erc20___CallBuilder.
     let* α6 := α2.["exec_input"] α5 in
     α6.["returns"].
   
-  Global Instance Method_balance_of `{H : State.Trait} :
-    Notation.Dot "balance_of" := {
+  Global Instance Method_balance_of : Notation.Dot "balance_of" := {
     Notation.dot := balance_of;
   }.
   
   Definition allowance
-      `{H : State.Trait}
       (self : ref Self)
       (__ink_binding_0 : erc20.erc20.AccountId)
       (__ink_binding_1 : erc20.erc20.AccountId)
       :
-        M (H := H)
+        M
           (ink_env.call.call_builder.CallBuilder
             erc20.erc20.Environment
             (ink_env.call.common.Set
@@ -4372,7 +3936,7 @@ Module Impl_erc20_erc20___CallBuilder.
                     ink_env.call.execution_input.EmptyArgumentList))))
             (ink_env.call.common.Set
               (ink_env.call.common.ReturnType erc20.erc20.Balance))) :=
-    let* α0 := ink_env.call.call_builder.build_call tt in
+    let* α0 := ink_env.call.call_builder.build_call  in
     let* α1 := ink.contract_ref.ToAccountId.to_account_id self in
     let* α2 := α0.["call"] α1 in
     let* α3 := ink_env.call.selector.Selector::["new"] [ 106; 0; 22; 94 ] in
@@ -4382,18 +3946,16 @@ Module Impl_erc20_erc20___CallBuilder.
     let* α7 := α2.["exec_input"] α6 in
     α7.["returns"].
   
-  Global Instance Method_allowance `{H : State.Trait} :
-    Notation.Dot "allowance" := {
+  Global Instance Method_allowance : Notation.Dot "allowance" := {
     Notation.dot := allowance;
   }.
   
   Definition transfer
-      `{H : State.Trait}
       (self : mut_ref Self)
       (__ink_binding_0 : erc20.erc20.AccountId)
       (__ink_binding_1 : erc20.erc20.Balance)
       :
-        M (H := H)
+        M
           (ink_env.call.call_builder.CallBuilder
             erc20.erc20.Environment
             (ink_env.call.common.Set
@@ -4408,7 +3970,7 @@ Module Impl_erc20_erc20___CallBuilder.
                     ink_env.call.execution_input.EmptyArgumentList))))
             (ink_env.call.common.Set
               (ink_env.call.common.ReturnType (erc20.erc20.Result unit)))) :=
-    let* α0 := ink_env.call.call_builder.build_call tt in
+    let* α0 := ink_env.call.call_builder.build_call  in
     let* α1 := ink.contract_ref.ToAccountId.to_account_id self in
     let* α2 := α0.["call"] α1 in
     let* α3 := ink_env.call.selector.Selector::["new"] [ 132; 161; 93; 161 ] in
@@ -4418,18 +3980,16 @@ Module Impl_erc20_erc20___CallBuilder.
     let* α7 := α2.["exec_input"] α6 in
     α7.["returns"].
   
-  Global Instance Method_transfer `{H : State.Trait} :
-    Notation.Dot "transfer" := {
+  Global Instance Method_transfer : Notation.Dot "transfer" := {
     Notation.dot := transfer;
   }.
   
   Definition approve
-      `{H : State.Trait}
       (self : mut_ref Self)
       (__ink_binding_0 : erc20.erc20.AccountId)
       (__ink_binding_1 : erc20.erc20.Balance)
       :
-        M (H := H)
+        M
           (ink_env.call.call_builder.CallBuilder
             erc20.erc20.Environment
             (ink_env.call.common.Set
@@ -4444,7 +4004,7 @@ Module Impl_erc20_erc20___CallBuilder.
                     ink_env.call.execution_input.EmptyArgumentList))))
             (ink_env.call.common.Set
               (ink_env.call.common.ReturnType (erc20.erc20.Result unit)))) :=
-    let* α0 := ink_env.call.call_builder.build_call tt in
+    let* α0 := ink_env.call.call_builder.build_call  in
     let* α1 := ink.contract_ref.ToAccountId.to_account_id self in
     let* α2 := α0.["call"] α1 in
     let* α3 := ink_env.call.selector.Selector::["new"] [ 104; 18; 102; 160 ] in
@@ -4454,19 +4014,17 @@ Module Impl_erc20_erc20___CallBuilder.
     let* α7 := α2.["exec_input"] α6 in
     α7.["returns"].
   
-  Global Instance Method_approve `{H : State.Trait} :
-    Notation.Dot "approve" := {
+  Global Instance Method_approve : Notation.Dot "approve" := {
     Notation.dot := approve;
   }.
   
   Definition transfer_from
-      `{H : State.Trait}
       (self : mut_ref Self)
       (__ink_binding_0 : erc20.erc20.AccountId)
       (__ink_binding_1 : erc20.erc20.AccountId)
       (__ink_binding_2 : erc20.erc20.Balance)
       :
-        M (H := H)
+        M
           (ink_env.call.call_builder.CallBuilder
             erc20.erc20.Environment
             (ink_env.call.common.Set
@@ -4484,7 +4042,7 @@ Module Impl_erc20_erc20___CallBuilder.
                       ink_env.call.execution_input.EmptyArgumentList)))))
             (ink_env.call.common.Set
               (ink_env.call.common.ReturnType (erc20.erc20.Result unit)))) :=
-    let* α0 := ink_env.call.call_builder.build_call tt in
+    let* α0 := ink_env.call.call_builder.build_call  in
     let* α1 := ink.contract_ref.ToAccountId.to_account_id self in
     let* α2 := α0.["call"] α1 in
     let* α3 := ink_env.call.selector.Selector::["new"] [ 11; 57; 111; 24 ] in
@@ -4495,8 +4053,7 @@ Module Impl_erc20_erc20___CallBuilder.
     let* α8 := α2.["exec_input"] α7 in
     α8.["returns"].
   
-  Global Instance Method_transfer_from `{H : State.Trait} :
-    Notation.Dot "transfer_from" := {
+  Global Instance Method_transfer_from : Notation.Dot "transfer_from" := {
     Notation.dot := transfer_from;
   }.
 End Impl_erc20_erc20___CallBuilder.
@@ -4515,31 +4072,22 @@ Definition Erc20Ref : Set := Erc20Ref.t.
 Module Impl_core_fmt_Debug_for_erc20_erc20_Erc20Ref.
   Definition Self := erc20.erc20.Erc20Ref.
   
-  Parameter debug_struct_field1_finish : core.fmt.Formatter -> string -> 
-    string -> ink_codegen_dispatch_info_ContractCallBuilder_Type -> 
-    M (H := H) core.fmt.Result.
-  
-  Global Instance Deb_debug_struct_field1_finish : Notation.DoubleColon
-    core.fmt.Formatter "debug_struct_field1_finish" := {
-    Notation.double_colon := debug_struct_field1_finish; }.
-  
   Definition fmt
-      `{H : State.Trait}
       (self : ref Self)
       (f : mut_ref core.fmt.Formatter)
-      : M (H := H) core.fmt.Result :=
+      : M core.fmt.Result :=
     core.fmt.Formatter::["debug_struct_field1_finish"]
       f
       "Erc20Ref"
       "inner"
       (addr_of (addr_of self.["inner"])).
   
-  Global Instance Method_fmt `{H : State.Trait} : Notation.Dot "fmt" := {
+  Global Instance Method_fmt : Notation.Dot "fmt" := {
     Notation.dot := fmt;
   }.
   
   Global Instance I : core.fmt.Debug.Trait Self := {
-    core.fmt.Debug.fmt `{H : State.Trait} := fmt;
+    core.fmt.Debug.fmt := fmt;
   }.
 End Impl_core_fmt_Debug_for_erc20_erc20_Erc20Ref.
 
@@ -4547,40 +4095,32 @@ Module Impl_parity_scale_codec_codec_Encode_for_erc20_erc20_Erc20Ref.
   Definition Self := erc20.erc20.Erc20Ref.
   
   Definition encode_to
-      `{H : State.Trait}
       (self : ref Self)
       (__codec_dest_edqy : mut_ref __CodecOutputEdqy)
-      : M (H := H) unit :=
+      : M unit :=
     parity_scale_codec.codec.Encode.encode_to
       (addr_of (addr_of self.["inner"]))
       __codec_dest_edqy.
   
-  Global Instance Method_encode_to `{H : State.Trait} :
-    Notation.Dot "encode_to" := {
+  Global Instance Method_encode_to : Notation.Dot "encode_to" := {
     Notation.dot := encode_to;
   }.
   
   Definition encode
-      `{H : State.Trait}
       (self : ref Self)
-      : M (H := H) (alloc.vec.Vec Root.core.primitive.u8) :=
+      : M (alloc.vec.Vec Root.core.primitive.u8) :=
     parity_scale_codec.codec.Encode.encode (addr_of (addr_of self.["inner"])).
   
-  Global Instance Method_encode `{H : State.Trait} : Notation.Dot "encode" := {
+  Global Instance Method_encode : Notation.Dot "encode" := {
     Notation.dot := encode;
   }.
   
-  Definition using_encoded
-      `{H : State.Trait}
-      (self : ref Self)
-      (f : F)
-      : M (H := H) R :=
+  Definition using_encoded (self : ref Self) (f : F) : M R :=
     parity_scale_codec.codec.Encode.using_encoded
       (addr_of (addr_of self.["inner"]))
       f.
   
-  Global Instance Method_using_encoded `{H : State.Trait} :
-    Notation.Dot "using_encoded" := {
+  Global Instance Method_using_encoded : Notation.Dot "using_encoded" := {
     Notation.dot := using_encoded;
   }.
   
@@ -4599,9 +4139,8 @@ Module Impl_parity_scale_codec_codec_Decode_for_erc20_erc20_Erc20Ref.
   Definition Self := erc20.erc20.Erc20Ref.
   
   Definition decode
-      `{H : State.Trait}
       (__codec_input_edqy : mut_ref __CodecInputEdqy)
-      : M (H := H) (core.result.Result Self parity_scale_codec.error.Error) :=
+      : M (core.result.Result Self parity_scale_codec.error.Error) :=
     let* __codec_res_edqy :=
       parity_scale_codec.codec.Decode.decode __codec_input_edqy in
     let* α0 :=
@@ -4613,32 +4152,28 @@ Module Impl_parity_scale_codec_codec_Decode_for_erc20_erc20_Erc20Ref.
       end in
     Pure (core.result.Result.Ok {| erc20.erc20.Erc20Ref.inner := α0; |}).
   
-  Global Instance AssociatedFunction_decode `{H : State.Trait} :
+  Global Instance AssociatedFunction_decode :
     Notation.DoubleColon Self "decode" := {
     Notation.double_colon := decode;
   }.
   
   Global Instance I : parity_scale_codec.codec.Decode.Trait Self := {
-    parity_scale_codec.codec.Decode.decode `{H : State.Trait} := decode;
+    parity_scale_codec.codec.Decode.decode := decode;
   }.
 End Impl_parity_scale_codec_codec_Decode_for_erc20_erc20_Erc20Ref.
 
 Module Impl_core_hash_Hash_for_erc20_erc20_Erc20Ref.
   Definition Self := erc20.erc20.Erc20Ref.
   
-  Definition hash
-      `{H : State.Trait}
-      (self : ref Self)
-      (state : mut_ref __H)
-      : M (H := H) unit :=
+  Definition hash (self : ref Self) (state : mut_ref __H) : M unit :=
     core.hash.Hash.hash (addr_of self.["inner"]) state.
   
-  Global Instance Method_hash `{H : State.Trait} : Notation.Dot "hash" := {
+  Global Instance Method_hash : Notation.Dot "hash" := {
     Notation.dot := hash;
   }.
   
   Global Instance I : core.hash.Hash.Trait Self := {
-    core.hash.Hash.hash `{H : State.Trait} := hash;
+    core.hash.Hash.hash := hash;
   }.
 End Impl_core_hash_Hash_for_erc20_erc20_Erc20Ref.
 
@@ -4652,19 +4187,15 @@ End Impl_core_marker_StructuralPartialEq_for_erc20_erc20_Erc20Ref.
 Module Impl_core_cmp_PartialEq_for_erc20_erc20_Erc20Ref.
   Definition Self := erc20.erc20.Erc20Ref.
   
-  Definition eq
-      `{H : State.Trait}
-      (self : ref Self)
-      (other : ref erc20.erc20.Erc20Ref)
-      : M (H := H) bool :=
+  Definition eq (self : ref Self) (other : ref erc20.erc20.Erc20Ref) : M bool :=
     self.["inner"].["eq"] other.["inner"].
   
-  Global Instance Method_eq `{H : State.Trait} : Notation.Dot "eq" := {
+  Global Instance Method_eq : Notation.Dot "eq" := {
     Notation.dot := eq;
   }.
   
   Global Instance I : core.cmp.PartialEq.Trait Self := {
-    core.cmp.PartialEq.eq `{H : State.Trait} := eq;
+    core.cmp.PartialEq.eq := eq;
   }.
 End Impl_core_cmp_PartialEq_for_erc20_erc20_Erc20Ref.
 
@@ -4678,14 +4209,11 @@ End Impl_core_marker_StructuralEq_for_erc20_erc20_Erc20Ref.
 Module Impl_core_cmp_Eq_for_erc20_erc20_Erc20Ref.
   Definition Self := erc20.erc20.Erc20Ref.
   
-  Definition assert_receiver_is_total_eq
-      `{H : State.Trait}
-      (self : ref Self)
-      : M (H := H) unit :=
+  Definition assert_receiver_is_total_eq (self : ref Self) : M unit :=
     let _ := tt in
     Pure tt.
   
-  Global Instance Method_assert_receiver_is_total_eq `{H : State.Trait} :
+  Global Instance Method_assert_receiver_is_total_eq :
     Notation.Dot "assert_receiver_is_total_eq" := {
     Notation.dot := assert_receiver_is_total_eq;
   }.
@@ -4697,19 +4225,16 @@ End Impl_core_cmp_Eq_for_erc20_erc20_Erc20Ref.
 Module Impl_core_clone_Clone_for_erc20_erc20_Erc20Ref.
   Definition Self := erc20.erc20.Erc20Ref.
   
-  Definition clone
-      `{H : State.Trait}
-      (self : ref Self)
-      : M (H := H) erc20.erc20.Erc20Ref :=
+  Definition clone (self : ref Self) : M erc20.erc20.Erc20Ref :=
     let* α0 := core.clone.Clone.clone (addr_of self.["inner"]) in
     Pure {| erc20.erc20.Erc20Ref.inner := α0; |}.
   
-  Global Instance Method_clone `{H : State.Trait} : Notation.Dot "clone" := {
+  Global Instance Method_clone : Notation.Dot "clone" := {
     Notation.dot := clone;
   }.
   
   Global Instance I : core.clone.Clone.Trait Self := {
-    core.clone.Clone.clone `{H : State.Trait} := clone;
+    core.clone.Clone.clone := clone;
   }.
 End Impl_core_clone_Clone_for_erc20_erc20_Erc20Ref.
 
@@ -4718,17 +4243,14 @@ Module Impl_scale_info_TypeInfo_for_erc20_erc20_Erc20Ref.
   
   Definition Identity : Set := Self.
   
-  Definition type_info
-      `{H : State.Trait}
-      (_ : unit)
-      : M (H := H) scale_info.ty.Type :=
-    let* α0 := scale_info.ty.Type::["builder"] tt in
+  Definition type_info  : M scale_info.ty.Type :=
+    let* α0 := scale_info.ty.Type::["builder"]  in
     let* α1 := scale_info.ty.path.Path::["new"] "Erc20Ref" "erc20::erc20" in
     let* α2 := α0.["path"] α1 in
-    let* α3 := alloc.vec.Vec::["new"] tt in
+    let* α3 := alloc.vec.Vec::["new"]  in
     let* α4 := α2.["type_params"] α3 in
     let* α5 := α4.["docs"] (addr_of [ "A simple ERC-20 contract." ]) in
-    let* α6 := scale_info.build.Fields::["named"] tt in
+    let* α6 := scale_info.build.Fields::["named"]  in
     let* α7 :=
       α6.["field"]
         (fun f =>
@@ -4738,13 +4260,13 @@ Module Impl_scale_info_TypeInfo_for_erc20_erc20_Erc20Ref.
             "<Erc20 as::ink::codegen::ContractCallBuilder>::Type") in
     α5.["composite"] α7.
   
-  Global Instance AssociatedFunction_type_info `{H : State.Trait} :
+  Global Instance AssociatedFunction_type_info :
     Notation.DoubleColon Self "type_info" := {
     Notation.double_colon := type_info;
   }.
   
   Global Instance I : scale_info.TypeInfo.Trait Self := {
-    scale_info.TypeInfo.type_info `{H : State.Trait} := type_info;
+    scale_info.TypeInfo.type_info := type_info;
   }.
 End Impl_scale_info_TypeInfo_for_erc20_erc20_Erc20Ref.
 
@@ -4752,21 +4274,20 @@ Module Impl_ink_storage_traits_layout_StorageLayout_for_erc20_erc20_Erc20Ref.
   Definition Self := erc20.erc20.Erc20Ref.
   
   Definition layout
-      `{H : State.Trait}
       (__key : ref ink_primitives.key.Key)
-      : M (H := H) ink_metadata.layout.Layout :=
+      : M ink_metadata.layout.Layout :=
     let* α0 := ink_storage_traits.layout.StorageLayout.layout __key in
     let* α1 := ink_metadata.layout.FieldLayout::["new"] "inner" α0 in
     let* α2 := ink_metadata.layout.StructLayout::["new"] "Erc20Ref" [ α1 ] in
     Pure (ink_metadata.layout.Layout.Struct α2).
   
-  Global Instance AssociatedFunction_layout `{H : State.Trait} :
+  Global Instance AssociatedFunction_layout :
     Notation.DoubleColon Self "layout" := {
     Notation.double_colon := layout;
   }.
   
   Global Instance I : ink_storage_traits.layout.StorageLayout.Trait Self := {
-    ink_storage_traits.layout.StorageLayout.layout `{H : State.Trait} := layout;
+    ink_storage_traits.layout.StorageLayout.layout := layout;
   }.
 End Impl_ink_storage_traits_layout_StorageLayout_for_erc20_erc20_Erc20Ref.
 
@@ -4787,14 +4308,10 @@ Module
   
   Definition Error : Set := unit.
   
-  Definition ok
-      `{H : State.Trait}
-      (value : erc20.erc20.Erc20Ref)
-      : M (H := H) ImplSelf.Output :=
+  Definition ok (value : erc20.erc20.Erc20Ref) : M ImplSelf.Output :=
     Pure value.
   
-  Global Instance AssociatedFunction_ok `{H : State.Trait} :
-    Notation.DoubleColon Self "ok" := {
+  Global Instance AssociatedFunction_ok : Notation.DoubleColon Self "ok" := {
     Notation.double_colon := ok;
   }.
   
@@ -4802,10 +4319,7 @@ Module
       ink_env.call.create_builder.ConstructorReturnType.Trait
         Self
         (C := erc20.erc20.Erc20Ref) := {
-    ink_env.call.create_builder.ConstructorReturnType.ok
-      `{H : State.Trait}
-      :=
-      ok;
+    ink_env.call.create_builder.ConstructorReturnType.ok := ok;
   }.
 End
   Impl_ink_env_call_create_builder_ConstructorReturnType_for_erc20_erc20_Erc20.
@@ -4820,7 +4334,7 @@ Section
   
   Definition IS_RESULT := Pure true.
   
-  Global Instance AssociatedFunction_IS_RESULT `{H : State.Trait} :
+  Global Instance AssociatedFunction_IS_RESULT :
     Notation.DoubleColon Self "IS_RESULT" := {
     Notation.double_colon := IS_RESULT;
   }.
@@ -4829,25 +4343,19 @@ Section
   
   Definition Error : Set := E.
   
-  Definition ok
-      `{H : State.Trait}
-      (value : erc20.erc20.Erc20Ref)
-      : M (H := H) ImplSelf.Output :=
+  Definition ok (value : erc20.erc20.Erc20Ref) : M ImplSelf.Output :=
     Pure (core.result.Result.Ok value).
   
-  Global Instance AssociatedFunction_ok `{H : State.Trait} :
-    Notation.DoubleColon Self "ok" := {
+  Global Instance AssociatedFunction_ok : Notation.DoubleColon Self "ok" := {
     Notation.double_colon := ok;
   }.
   
   Definition err
-      `{H : State.Trait}
       (err : ImplSelf.Error)
-      : M (H := H) (core.option.Option ImplSelf.Output) :=
+      : M (core.option.Option ImplSelf.Output) :=
     Pure (core.option.Option.Some (core.result.Result.Err err)).
   
-  Global Instance AssociatedFunction_err `{H : State.Trait} :
-    Notation.DoubleColon Self "err" := {
+  Global Instance AssociatedFunction_err : Notation.DoubleColon Self "err" := {
     Notation.double_colon := err;
   }.
   
@@ -4855,10 +4363,7 @@ Section
       ink_env.call.create_builder.ConstructorReturnType.Trait
         Self
         (C := erc20.erc20.Erc20Ref) := {
-    ink_env.call.create_builder.ConstructorReturnType.ok
-      `{H : State.Trait}
-      :=
-      ok;
+    ink_env.call.create_builder.ConstructorReturnType.ok := ok;
   }.
 End
   Impl_ink_env_call_create_builder_ConstructorReturnType_for_core_result_Result_erc20_erc20_Erc20_E.
@@ -4878,10 +4383,9 @@ Module Impl_erc20_erc20_Erc20Ref_2.
   Definition Self := erc20.erc20.Erc20Ref.
   
   Definition new
-      `{H : State.Trait}
       (__ink_binding_0 : erc20.erc20.Balance)
       :
-        M (H := H)
+        M
           (ink_env.call.create_builder.CreateBuilder
             erc20.erc20.Environment
             Self
@@ -4895,22 +4399,18 @@ Module Impl_erc20_erc20_Erc20Ref_2.
                   ink_env.call.execution_input.EmptyArgumentList)))
             (ink_env.call.common.Unset ink_env.call.create_builder.state.Salt)
             (ink_env.call.common.Set (ink_env.call.common.ReturnType Self))) :=
-    let* α0 := ink_env.call.create_builder.build_create tt in
+    let* α0 := ink_env.call.create_builder.build_create  in
     let* α1 := ink_env.call.selector.Selector::["new"] [ 155; 174; 157; 94 ] in
     let* α2 := ink_env.call.execution_input.ExecutionInput::["new"] α1 in
     let* α3 := α2.["push_arg"] __ink_binding_0 in
     let* α4 := α0.["exec_input"] α3 in
     α4.["returns"].
   
-  Global Instance AssociatedFunction_new `{H : State.Trait} :
-    Notation.DoubleColon Self "new" := {
+  Global Instance AssociatedFunction_new : Notation.DoubleColon Self "new" := {
     Notation.double_colon := new;
   }.
   
-  Definition total_supply
-      `{H : State.Trait}
-      (self : ref Self)
-      : M (H := H) erc20.erc20.Balance :=
+  Definition total_supply (self : ref Self) : M erc20.erc20.Balance :=
     let* α0 := self.["try_total_supply"] in
     α0.["unwrap_or_else"]
       (fun error =>
@@ -4922,15 +4422,13 @@ Module Impl_erc20_erc20_Erc20Ref_2.
             (addr_of [ α0 ]) in
         core.panicking.panic_fmt α1).
   
-  Global Instance Method_total_supply `{H : State.Trait} :
-    Notation.Dot "total_supply" := {
+  Global Instance Method_total_supply : Notation.Dot "total_supply" := {
     Notation.dot := total_supply;
   }.
   
   Definition try_total_supply
-      `{H : State.Trait}
       (self : ref Self)
-      : M (H := H) (ink_primitives.MessageResult erc20.erc20.Balance) :=
+      : M (ink_primitives.MessageResult erc20.erc20.Balance) :=
     let* α0 := ink.codegen.trait_def.call_builder.TraitCallBuilder.call self in
     let* α1 := α0.["total_supply"] in
     let* α2 := α1.["try_invoke"] in
@@ -4944,16 +4442,14 @@ Module Impl_erc20_erc20_Erc20Ref_2.
             (addr_of [ α0 ]) in
         core.panicking.panic_fmt α1).
   
-  Global Instance Method_try_total_supply `{H : State.Trait} :
-    Notation.Dot "try_total_supply" := {
+  Global Instance Method_try_total_supply : Notation.Dot "try_total_supply" := {
     Notation.dot := try_total_supply;
   }.
   
   Definition balance_of
-      `{H : State.Trait}
       (self : ref Self)
       (owner : erc20.erc20.AccountId)
-      : M (H := H) erc20.erc20.Balance :=
+      : M erc20.erc20.Balance :=
     let* α0 := self.["try_balance_of"] owner in
     α0.["unwrap_or_else"]
       (fun error =>
@@ -4964,16 +4460,14 @@ Module Impl_erc20_erc20_Erc20Ref_2.
             (addr_of [ α0 ]) in
         core.panicking.panic_fmt α1).
   
-  Global Instance Method_balance_of `{H : State.Trait} :
-    Notation.Dot "balance_of" := {
+  Global Instance Method_balance_of : Notation.Dot "balance_of" := {
     Notation.dot := balance_of;
   }.
   
   Definition try_balance_of
-      `{H : State.Trait}
       (self : ref Self)
       (owner : erc20.erc20.AccountId)
-      : M (H := H) (ink_primitives.MessageResult erc20.erc20.Balance) :=
+      : M (ink_primitives.MessageResult erc20.erc20.Balance) :=
     let* α0 := ink.codegen.trait_def.call_builder.TraitCallBuilder.call self in
     let* α1 := α0.["balance_of"] owner in
     let* α2 := α1.["try_invoke"] in
@@ -4986,17 +4480,15 @@ Module Impl_erc20_erc20_Erc20Ref_2.
             (addr_of [ α0 ]) in
         core.panicking.panic_fmt α1).
   
-  Global Instance Method_try_balance_of `{H : State.Trait} :
-    Notation.Dot "try_balance_of" := {
+  Global Instance Method_try_balance_of : Notation.Dot "try_balance_of" := {
     Notation.dot := try_balance_of;
   }.
   
   Definition allowance
-      `{H : State.Trait}
       (self : ref Self)
       (owner : erc20.erc20.AccountId)
       (spender : erc20.erc20.AccountId)
-      : M (H := H) erc20.erc20.Balance :=
+      : M erc20.erc20.Balance :=
     let* α0 := self.["try_allowance"] owner spender in
     α0.["unwrap_or_else"]
       (fun error =>
@@ -5007,17 +4499,15 @@ Module Impl_erc20_erc20_Erc20Ref_2.
             (addr_of [ α0 ]) in
         core.panicking.panic_fmt α1).
   
-  Global Instance Method_allowance `{H : State.Trait} :
-    Notation.Dot "allowance" := {
+  Global Instance Method_allowance : Notation.Dot "allowance" := {
     Notation.dot := allowance;
   }.
   
   Definition try_allowance
-      `{H : State.Trait}
       (self : ref Self)
       (owner : erc20.erc20.AccountId)
       (spender : erc20.erc20.AccountId)
-      : M (H := H) (ink_primitives.MessageResult erc20.erc20.Balance) :=
+      : M (ink_primitives.MessageResult erc20.erc20.Balance) :=
     let* α0 := ink.codegen.trait_def.call_builder.TraitCallBuilder.call self in
     let* α1 := α0.["allowance"] owner spender in
     let* α2 := α1.["try_invoke"] in
@@ -5030,17 +4520,15 @@ Module Impl_erc20_erc20_Erc20Ref_2.
             (addr_of [ α0 ]) in
         core.panicking.panic_fmt α1).
   
-  Global Instance Method_try_allowance `{H : State.Trait} :
-    Notation.Dot "try_allowance" := {
+  Global Instance Method_try_allowance : Notation.Dot "try_allowance" := {
     Notation.dot := try_allowance;
   }.
   
   Definition transfer
-      `{H : State.Trait}
       (self : mut_ref Self)
       (to : erc20.erc20.AccountId)
       (value : erc20.erc20.Balance)
-      : M (H := H) (erc20.erc20.Result unit) :=
+      : M (erc20.erc20.Result unit) :=
     let* α0 := self.["try_transfer"] to value in
     α0.["unwrap_or_else"]
       (fun error =>
@@ -5051,17 +4539,15 @@ Module Impl_erc20_erc20_Erc20Ref_2.
             (addr_of [ α0 ]) in
         core.panicking.panic_fmt α1).
   
-  Global Instance Method_transfer `{H : State.Trait} :
-    Notation.Dot "transfer" := {
+  Global Instance Method_transfer : Notation.Dot "transfer" := {
     Notation.dot := transfer;
   }.
   
   Definition try_transfer
-      `{H : State.Trait}
       (self : mut_ref Self)
       (to : erc20.erc20.AccountId)
       (value : erc20.erc20.Balance)
-      : M (H := H) (ink_primitives.MessageResult (erc20.erc20.Result unit)) :=
+      : M (ink_primitives.MessageResult (erc20.erc20.Result unit)) :=
     let* α0 :=
       ink.codegen.trait_def.call_builder.TraitCallBuilder.call_mut self in
     let* α1 := α0.["transfer"] to value in
@@ -5075,17 +4561,15 @@ Module Impl_erc20_erc20_Erc20Ref_2.
             (addr_of [ α0 ]) in
         core.panicking.panic_fmt α1).
   
-  Global Instance Method_try_transfer `{H : State.Trait} :
-    Notation.Dot "try_transfer" := {
+  Global Instance Method_try_transfer : Notation.Dot "try_transfer" := {
     Notation.dot := try_transfer;
   }.
   
   Definition approve
-      `{H : State.Trait}
       (self : mut_ref Self)
       (spender : erc20.erc20.AccountId)
       (value : erc20.erc20.Balance)
-      : M (H := H) (erc20.erc20.Result unit) :=
+      : M (erc20.erc20.Result unit) :=
     let* α0 := self.["try_approve"] spender value in
     α0.["unwrap_or_else"]
       (fun error =>
@@ -5096,17 +4580,15 @@ Module Impl_erc20_erc20_Erc20Ref_2.
             (addr_of [ α0 ]) in
         core.panicking.panic_fmt α1).
   
-  Global Instance Method_approve `{H : State.Trait} :
-    Notation.Dot "approve" := {
+  Global Instance Method_approve : Notation.Dot "approve" := {
     Notation.dot := approve;
   }.
   
   Definition try_approve
-      `{H : State.Trait}
       (self : mut_ref Self)
       (spender : erc20.erc20.AccountId)
       (value : erc20.erc20.Balance)
-      : M (H := H) (ink_primitives.MessageResult (erc20.erc20.Result unit)) :=
+      : M (ink_primitives.MessageResult (erc20.erc20.Result unit)) :=
     let* α0 :=
       ink.codegen.trait_def.call_builder.TraitCallBuilder.call_mut self in
     let* α1 := α0.["approve"] spender value in
@@ -5120,18 +4602,16 @@ Module Impl_erc20_erc20_Erc20Ref_2.
             (addr_of [ α0 ]) in
         core.panicking.panic_fmt α1).
   
-  Global Instance Method_try_approve `{H : State.Trait} :
-    Notation.Dot "try_approve" := {
+  Global Instance Method_try_approve : Notation.Dot "try_approve" := {
     Notation.dot := try_approve;
   }.
   
   Definition transfer_from
-      `{H : State.Trait}
       (self : mut_ref Self)
       (from : erc20.erc20.AccountId)
       (to : erc20.erc20.AccountId)
       (value : erc20.erc20.Balance)
-      : M (H := H) (erc20.erc20.Result unit) :=
+      : M (erc20.erc20.Result unit) :=
     let* α0 := self.["try_transfer_from"] from to value in
     α0.["unwrap_or_else"]
       (fun error =>
@@ -5143,18 +4623,16 @@ Module Impl_erc20_erc20_Erc20Ref_2.
             (addr_of [ α0 ]) in
         core.panicking.panic_fmt α1).
   
-  Global Instance Method_transfer_from `{H : State.Trait} :
-    Notation.Dot "transfer_from" := {
+  Global Instance Method_transfer_from : Notation.Dot "transfer_from" := {
     Notation.dot := transfer_from;
   }.
   
   Definition try_transfer_from
-      `{H : State.Trait}
       (self : mut_ref Self)
       (from : erc20.erc20.AccountId)
       (to : erc20.erc20.AccountId)
       (value : erc20.erc20.Balance)
-      : M (H := H) (ink_primitives.MessageResult (erc20.erc20.Result unit)) :=
+      : M (ink_primitives.MessageResult (erc20.erc20.Result unit)) :=
     let* α0 :=
       ink.codegen.trait_def.call_builder.TraitCallBuilder.call_mut self in
     let* α1 := α0.["transfer_from"] from to value in
@@ -5169,7 +4647,7 @@ Module Impl_erc20_erc20_Erc20Ref_2.
             (addr_of [ α0 ]) in
         core.panicking.panic_fmt α1).
   
-  Global Instance Method_try_transfer_from `{H : State.Trait} :
+  Global Instance Method_try_transfer_from :
     Notation.Dot "try_transfer_from" := {
     Notation.dot := try_transfer_from;
   }.
@@ -5182,37 +4660,24 @@ Module
   Definition Builder : Set :=
     ink.codegen.dispatch.info.ContractCallBuilder.Type.
   
-  Definition call
-      `{H : State.Trait}
-      (self : ref Self)
-      : M (H := H) (ref ImplSelf.Builder) :=
+  Definition call (self : ref Self) : M (ref ImplSelf.Builder) :=
     Pure (addr_of self.["inner"]).
   
-  Global Instance Method_call `{H : State.Trait} : Notation.Dot "call" := {
+  Global Instance Method_call : Notation.Dot "call" := {
     Notation.dot := call;
   }.
   
-  Definition call_mut
-      `{H : State.Trait}
-      (self : mut_ref Self)
-      : M (H := H) (mut_ref ImplSelf.Builder) :=
+  Definition call_mut (self : mut_ref Self) : M (mut_ref ImplSelf.Builder) :=
     Pure (addr_of self.["inner"]).
   
-  Global Instance Method_call_mut `{H : State.Trait} :
-    Notation.Dot "call_mut" := {
+  Global Instance Method_call_mut : Notation.Dot "call_mut" := {
     Notation.dot := call_mut;
   }.
   
   Global Instance I :
       ink.codegen.trait_def.call_builder.TraitCallBuilder.Trait Self := {
-    ink.codegen.trait_def.call_builder.TraitCallBuilder.call
-      `{H : State.Trait}
-      :=
-      call;
-    ink.codegen.trait_def.call_builder.TraitCallBuilder.call_mut
-      `{H : State.Trait}
-      :=
-      call_mut;
+    ink.codegen.trait_def.call_builder.TraitCallBuilder.call := call;
+    ink.codegen.trait_def.call_builder.TraitCallBuilder.call_mut := call_mut;
   }.
 End
   Impl_ink_codegen_trait_def_call_builder_TraitCallBuilder_for_erc20_erc20_Erc20Ref.
@@ -5220,15 +4685,12 @@ End
 Module Impl_ink_env_call_create_builder_FromAccountId_for_erc20_erc20_Erc20Ref.
   Definition Self := erc20.erc20.Erc20Ref.
   
-  Definition from_account_id
-      `{H : State.Trait}
-      (account_id : erc20.erc20.AccountId)
-      : M (H := H) Self :=
+  Definition from_account_id (account_id : erc20.erc20.AccountId) : M Self :=
     let* α0 :=
       ink_env.call.create_builder.FromAccountId.from_account_id account_id in
     Pure {| Self.inner := α0; |}.
   
-  Global Instance AssociatedFunction_from_account_id `{H : State.Trait} :
+  Global Instance AssociatedFunction_from_account_id :
     Notation.DoubleColon Self "from_account_id" := {
     Notation.double_colon := from_account_id;
   }.
@@ -5238,7 +4700,6 @@ Module Impl_ink_env_call_create_builder_FromAccountId_for_erc20_erc20_Erc20Ref.
         Self
         (T := erc20.erc20.Environment) := {
     ink_env.call.create_builder.FromAccountId.from_account_id
-      `{H : State.Trait}
       :=
       from_account_id;
   }.
@@ -5247,14 +4708,10 @@ End Impl_ink_env_call_create_builder_FromAccountId_for_erc20_erc20_Erc20Ref.
 Module Impl_ink_contract_ref_ToAccountId_for_erc20_erc20_Erc20Ref.
   Definition Self := erc20.erc20.Erc20Ref.
   
-  Definition to_account_id
-      `{H : State.Trait}
-      (self : ref Self)
-      : M (H := H) erc20.erc20.AccountId :=
+  Definition to_account_id (self : ref Self) : M erc20.erc20.AccountId :=
     ink.contract_ref.ToAccountId.to_account_id (addr_of self.["inner"]).
   
-  Global Instance Method_to_account_id `{H : State.Trait} :
-    Notation.Dot "to_account_id" := {
+  Global Instance Method_to_account_id : Notation.Dot "to_account_id" := {
     Notation.dot := to_account_id;
   }.
   
@@ -5262,55 +4719,43 @@ Module Impl_ink_contract_ref_ToAccountId_for_erc20_erc20_Erc20Ref.
       ink.contract_ref.ToAccountId.Trait
         Self
         (T := erc20.erc20.Environment) := {
-    ink.contract_ref.ToAccountId.to_account_id
-      `{H : State.Trait}
-      :=
-      to_account_id;
+    ink.contract_ref.ToAccountId.to_account_id := to_account_id;
   }.
 End Impl_ink_contract_ref_ToAccountId_for_erc20_erc20_Erc20Ref.
 
 Module Impl_core_convert_AsRef_for_erc20_erc20_Erc20Ref.
   Definition Self := erc20.erc20.Erc20Ref.
   
-  Definition as_ref
-      `{H : State.Trait}
-      (self : ref Self)
-      : M (H := H) (ref erc20.erc20.AccountId) :=
+  Definition as_ref (self : ref Self) : M (ref erc20.erc20.AccountId) :=
     core.convert.AsRef.as_ref (addr_of self.["inner"]).
   
-  Global Instance Method_as_ref `{H : State.Trait} : Notation.Dot "as_ref" := {
+  Global Instance Method_as_ref : Notation.Dot "as_ref" := {
     Notation.dot := as_ref;
   }.
   
   Global Instance I :
       core.convert.AsRef.Trait Self (T := erc20.erc20.AccountId) := {
-    core.convert.AsRef.as_ref `{H : State.Trait} := as_ref;
+    core.convert.AsRef.as_ref := as_ref;
   }.
 End Impl_core_convert_AsRef_for_erc20_erc20_Erc20Ref.
 
 Module Impl_core_convert_AsMut_for_erc20_erc20_Erc20Ref.
   Definition Self := erc20.erc20.Erc20Ref.
   
-  Definition as_mut
-      `{H : State.Trait}
-      (self : mut_ref Self)
-      : M (H := H) (mut_ref erc20.erc20.AccountId) :=
+  Definition as_mut (self : mut_ref Self) : M (mut_ref erc20.erc20.AccountId) :=
     core.convert.AsMut.as_mut (addr_of self.["inner"]).
   
-  Global Instance Method_as_mut `{H : State.Trait} : Notation.Dot "as_mut" := {
+  Global Instance Method_as_mut : Notation.Dot "as_mut" := {
     Notation.dot := as_mut;
   }.
   
   Global Instance I :
       core.convert.AsMut.Trait Self (T := erc20.erc20.AccountId) := {
-    core.convert.AsMut.as_mut `{H : State.Trait} := as_mut;
+    core.convert.AsMut.as_mut := as_mut;
   }.
 End Impl_core_convert_AsMut_for_erc20_erc20_Erc20Ref.
 
-Definition __ink_generate_metadata
-    `{H : State.Trait}
-    (_ : unit)
-    : M (H := H) ink_metadata.InkProject :=
+Definition __ink_generate_metadata  : M ink_metadata.InkProject :=
   let* layout :=
     let* α0 :=
       core.convert.From.from ink_storage_traits.storage.StorageKey.KEY in
@@ -5331,7 +4776,7 @@ Definition __ink_generate_metadata
             (addr_of [ "metadata ink! generation failed: " ])
             (addr_of [ α0 ]) in
         core.panicking.panic_fmt α1) in
-  let* α0 := ink_metadata.specs.ContractSpec::["new"] tt in
+  let* α0 := ink_metadata.specs.ContractSpec::["new"]  in
   let* α1 := ink_metadata.specs.ConstructorSpec::["from_label"] "new" in
   let* α2 := α1.["selector"] [ 155; 174; 157; 94 ] in
   let* α3 := ink_metadata.specs.MessageParamSpec::["new"] "total_supply" in
@@ -5660,7 +5105,7 @@ Definition __ink_generate_metadata
     core.iter.traits.iterator.Iterator.map α215 core.convert.AsRef.as_ref in
   let* α217 := ink_metadata.specs.TypeSpec::["with_name_segs"] α216 in
   let* α218 := α214.["lang_error"] α217 in
-  let* α219 := ink_metadata.specs.EnvironmentSpec::["new"] tt in
+  let* α219 := ink_metadata.specs.EnvironmentSpec::["new"]  in
   let* α220 :=
     core.iter.traits.collect.IntoIterator.into_iter [ "AccountId" ] in
   let* α221 :=
@@ -5713,17 +5158,14 @@ Module Impl_scale_info_TypeInfo_for_erc20_erc20_Error.
   
   Definition Identity : Set := Self.
   
-  Definition type_info
-      `{H : State.Trait}
-      (_ : unit)
-      : M (H := H) scale_info.ty.Type :=
-    let* α0 := scale_info.ty.Type::["builder"] tt in
+  Definition type_info  : M scale_info.ty.Type :=
+    let* α0 := scale_info.ty.Type::["builder"]  in
     let* α1 := scale_info.ty.path.Path::["new"] "Error" "erc20::erc20" in
     let* α2 := α0.["path"] α1 in
-    let* α3 := alloc.vec.Vec::["new"] tt in
+    let* α3 := alloc.vec.Vec::["new"]  in
     let* α4 := α2.["type_params"] α3 in
     let* α5 := α4.["docs"] (addr_of [ "The ERC-20 error types." ]) in
-    let* α6 := scale_info.build.Variants::["new"] tt in
+    let* α6 := scale_info.build.Variants::["new"]  in
     let* α7 :=
       α6.["variant"]
         "InsufficientBalance"
@@ -5746,13 +5188,13 @@ Module Impl_scale_info_TypeInfo_for_erc20_erc20_Error.
               ])) in
     α5.["variant"] α8.
   
-  Global Instance AssociatedFunction_type_info `{H : State.Trait} :
+  Global Instance AssociatedFunction_type_info :
     Notation.DoubleColon Self "type_info" := {
     Notation.double_colon := type_info;
   }.
   
   Global Instance I : scale_info.TypeInfo.Trait Self := {
-    scale_info.TypeInfo.type_info `{H : State.Trait} := type_info;
+    scale_info.TypeInfo.type_info := type_info;
   }.
 End Impl_scale_info_TypeInfo_for_erc20_erc20_Error.
 
@@ -5760,10 +5202,9 @@ Module Impl_core_fmt_Debug_for_erc20_erc20_Error.
   Definition Self := erc20.erc20.Error.
   
   Definition fmt
-      `{H : State.Trait}
       (self : ref Self)
       (f : mut_ref core.fmt.Formatter)
-      : M (H := H) core.fmt.Result :=
+      : M core.fmt.Result :=
     let* α0 :=
       match self with
       | erc20.erc20.Error.InsufficientBalance => Pure "InsufficientBalance"
@@ -5771,12 +5212,12 @@ Module Impl_core_fmt_Debug_for_erc20_erc20_Error.
       end in
     core.fmt.Formatter::["write_str"] f α0.
   
-  Global Instance Method_fmt `{H : State.Trait} : Notation.Dot "fmt" := {
+  Global Instance Method_fmt : Notation.Dot "fmt" := {
     Notation.dot := fmt;
   }.
   
   Global Instance I : core.fmt.Debug.Trait Self := {
-    core.fmt.Debug.fmt `{H : State.Trait} := fmt;
+    core.fmt.Debug.fmt := fmt;
   }.
 End Impl_core_fmt_Debug_for_erc20_erc20_Error.
 
@@ -5790,21 +5231,17 @@ End Impl_core_marker_StructuralPartialEq_for_erc20_erc20_Error.
 Module Impl_core_cmp_PartialEq_for_erc20_erc20_Error.
   Definition Self := erc20.erc20.Error.
   
-  Definition eq
-      `{H : State.Trait}
-      (self : ref Self)
-      (other : ref erc20.erc20.Error)
-      : M (H := H) bool :=
+  Definition eq (self : ref Self) (other : ref erc20.erc20.Error) : M bool :=
     let* __self_tag := core.intrinsics.discriminant_value self in
     let* __arg1_tag := core.intrinsics.discriminant_value other in
     __self_tag.["eq"] __arg1_tag.
   
-  Global Instance Method_eq `{H : State.Trait} : Notation.Dot "eq" := {
+  Global Instance Method_eq : Notation.Dot "eq" := {
     Notation.dot := eq;
   }.
   
   Global Instance I : core.cmp.PartialEq.Trait Self := {
-    core.cmp.PartialEq.eq `{H : State.Trait} := eq;
+    core.cmp.PartialEq.eq := eq;
   }.
 End Impl_core_cmp_PartialEq_for_erc20_erc20_Error.
 
@@ -5818,13 +5255,9 @@ End Impl_core_marker_StructuralEq_for_erc20_erc20_Error.
 Module Impl_core_cmp_Eq_for_erc20_erc20_Error.
   Definition Self := erc20.erc20.Error.
   
-  Definition assert_receiver_is_total_eq
-      `{H : State.Trait}
-      (self : ref Self)
-      : M (H := H) unit :=
-    Pure tt.
+  Definition assert_receiver_is_total_eq (self : ref Self) : M unit := Pure tt.
   
-  Global Instance Method_assert_receiver_is_total_eq `{H : State.Trait} :
+  Global Instance Method_assert_receiver_is_total_eq :
     Notation.Dot "assert_receiver_is_total_eq" := {
     Notation.dot := assert_receiver_is_total_eq;
   }.
@@ -5837,10 +5270,9 @@ Module Impl_parity_scale_codec_codec_Encode_for_erc20_erc20_Error.
   Definition Self := erc20.erc20.Error.
   
   Definition encode_to
-      `{H : State.Trait}
       (self : ref Self)
       (__codec_dest_edqy : mut_ref __CodecOutputEdqy)
-      : M (H := H) unit :=
+      : M unit :=
     let* α0 := self.["deref"] in
     match α0 with
     | erc20.erc20.Error.InsufficientBalance =>
@@ -5854,8 +5286,7 @@ Module Impl_parity_scale_codec_codec_Encode_for_erc20_erc20_Error.
     | _ => Pure tt
     end.
   
-  Global Instance Method_encode_to `{H : State.Trait} :
-    Notation.Dot "encode_to" := {
+  Global Instance Method_encode_to : Notation.Dot "encode_to" := {
     Notation.dot := encode_to;
   }.
   
@@ -5874,9 +5305,8 @@ Module Impl_parity_scale_codec_codec_Decode_for_erc20_erc20_Error.
   Definition Self := erc20.erc20.Error.
   
   Definition decode
-      `{H : State.Trait}
       (__codec_input_edqy : mut_ref __CodecInputEdqy)
-      : M (H := H) (core.result.Result Self parity_scale_codec.error.Error) :=
+      : M (core.result.Result Self parity_scale_codec.error.Error) :=
     let* α0 := __codec_input_edqy.["read_byte"] in
     let* α1 :=
       α0.["map_err"]
@@ -5898,7 +5328,7 @@ Module Impl_parity_scale_codec_codec_Decode_for_erc20_erc20_Error.
           (fun  =>
               Pure
                 (core.result.Result.Ok erc20.erc20.Error.InsufficientBalance))
-            tt in
+             in
         Return α0 in
       Pure tt
     | __codec_x_edqy =>
@@ -5907,7 +5337,7 @@ Module Impl_parity_scale_codec_codec_Decode_for_erc20_erc20_Error.
           (fun  =>
               Pure
                 (core.result.Result.Ok erc20.erc20.Error.InsufficientAllowance))
-            tt in
+             in
         Return α0 in
       Pure tt
     | _ =>
@@ -5918,18 +5348,18 @@ Module Impl_parity_scale_codec_codec_Decode_for_erc20_erc20_Error.
                 core.convert.Into.into
                   "Could not decode `Error`, variant doesn't exist" in
               Pure (core.result.Result.Err α0))
-            tt in
+             in
         Return α0 in
       Pure tt
     end.
   
-  Global Instance AssociatedFunction_decode `{H : State.Trait} :
+  Global Instance AssociatedFunction_decode :
     Notation.DoubleColon Self "decode" := {
     Notation.double_colon := decode;
   }.
   
   Global Instance I : parity_scale_codec.codec.Decode.Trait Self := {
-    parity_scale_codec.codec.Decode.decode `{H : State.Trait} := decode;
+    parity_scale_codec.codec.Decode.decode := decode;
   }.
 End Impl_parity_scale_codec_codec_Decode_for_erc20_erc20_Error.
 
